bla

CaseStudies/ABP/ABP_TSPS.thy
@@ -6,7 +6,7 @@
 *)
 
 theory ABP_TSPS
-  imports  Receiver Composition Medium "../../timed/TSPF" "../../UFun_Comp" "../../UFun" "../../UBundle" "../../USpec"
+  imports  Sender Receiver Composition Medium "../../timed/TSPF" "../../UFun_Comp" "../../UFun" "../../UBundle" "../../USpec"
 
 begin
 
@@ -27,12 +27,12 @@ end
 instantiation MABP ::  (countable) message
 begin
 fun ctype_MABP :: "channel \<Rightarrow> 'a MABP set" where
-  "ctype_MABP abpIn = range Data" |
-  "ctype_MABP abpOut = range Data" |
-  "ctype_MABP ds = range BoolPair" |
-  "ctype_MABP dr = range BoolPair" |
-  "ctype_MABP as = range Bool" |
-  "ctype_MABP ar = range Bool" |
+  "ctype_MABP c_abpIn = range Data" |
+  "ctype_MABP c_abpOut = range Data" |
+  "ctype_MABP c_ds = range BoolPair" |
+  "ctype_MABP c_dr = range BoolPair" |
+  "ctype_MABP c_as = range Bool" |
+  "ctype_MABP c_ar = range Bool" |
   "ctype_MABP other = undefined"
 
   instance ..
@@ -58,50 +58,50 @@ abbreviation invData :: "'a MABP \<Rightarrow> 'a" where
 
 abbreviation recvAbb where
 "recvAbb \<equiv>
-let recRes = (\<lambda> x. tsRec\<cdot>((tsMap invBoolPair)\<cdot>(x . dr)))
-in (\<lambda> x. (ubDom\<cdot>x = {dr}) \<leadsto> Abs_ubundle([ar    \<mapsto> tsMap Bool\<cdot>(fst (recRes x)),
-                                        abpOut \<mapsto> tsMap Data\<cdot>(snd (recRes x))]))"
+let recRes = (\<lambda> x. tsRec\<cdot>((tsMap invBoolPair)\<cdot>(x . c_dr)))
+in (\<lambda> x. (ubclDom\<cdot>x = {c_dr}) \<leadsto> Abs_ubundle([c_ar    \<mapsto> tsMap Bool\<cdot>(fst (recRes x)),
+                                        c_abpOut \<mapsto> tsMap Data\<cdot>(snd (recRes x))]))"
 
 
 subsection \<open>receiver\<close>
 definition recvTSPF :: "('a MABP tstream\<^sup>\<Omega>, 'a MABP tstream\<^sup>\<Omega>) ufun" where
-"recvTSPF \<equiv> Abs_cufun (\<lambda> x. (ubDom\<cdot>x = {dr}) \<leadsto> Abs_ubundle([ar    \<mapsto> (tsMap::(bool \<Rightarrow> 'a MABP) \<Rightarrow> bool tstream \<rightarrow> 'a MABP tstream) Bool\<cdot>(fst ( tsRec\<cdot>((tsMap invBoolPair)\<cdot>(x . dr)))),
-                                        abpOut \<mapsto> (tsMap::('a \<Rightarrow> 'a MABP) \<Rightarrow> 'a tstream \<rightarrow> 'a MABP tstream) Data\<cdot>(snd ( tsRec\<cdot>((tsMap invBoolPair)\<cdot>(x . dr))))]))"
-(* 
+"recvTSPF \<equiv> Abs_cufun (\<lambda> x. (ubclDom\<cdot>x = {c_dr}) \<leadsto> Abs_ubundle([c_ar    \<mapsto> (tsMap::(bool \<Rightarrow> 'a MABP) \<Rightarrow> bool tstream \<rightarrow> 'a MABP tstream) Bool\<cdot>(fst ( tsRec\<cdot>((tsMap invBoolPair)\<cdot>(x . c_dr)))),
+                                        c_abpOut \<mapsto> (tsMap::('a \<Rightarrow> 'a MABP) \<Rightarrow> 'a tstream \<rightarrow> 'a MABP tstream) Data\<cdot>(snd ( tsRec\<cdot>((tsMap invBoolPair)\<cdot>(x . c_dr))))]))"
+
 subsection \<open>medium_rs\<close>
   (* medium from receiver to sender *)
-  (* input: ar, output: as, transport booleans *)
+  (* input: c_ar, output: c_as, transport booleans *)
 
-definition medRS_TSPF :: "bool stream \<Rightarrow> 'a MABP TSPF" where
-"medRS_TSPF bst\<equiv> Abs_CTSPF (\<lambda> x. (tsbDom\<cdot>x = {ar})
-                           \<leadsto> [as \<mapsto> (tsMap::(bool \<Rightarrow> 'a MABP) \<Rightarrow> bool tstream \<rightarrow> 'a MABP tstream) Bool\<cdot>(tsMed\<cdot>(tsMap invBool\<cdot>(x . ar))\<cdot>bst)]\<Omega>)"
+definition medRS_TSPF :: "bool stream \<Rightarrow> ('a MABP tstream\<^sup>\<Omega>, 'a MABP tstream\<^sup>\<Omega>) ufun" where
+"medRS_TSPF bst\<equiv> Abs_cufun (\<lambda> x. (ubclDom\<cdot>x = {c_ar})
+                           \<leadsto> Abs_ubundle([c_as \<mapsto> (tsMap::(bool \<Rightarrow> 'a MABP) \<Rightarrow> bool tstream \<rightarrow> 'a MABP tstream) Bool\<cdot>(tsMed\<cdot>(tsMap invBool\<cdot>(x . c_ar))\<cdot>bst)]))"
 
-abbreviation tsMedRSAbb  :: "bool stream \<Rightarrow> 'a MABP TSB \<Rightarrow> 'a MABP TSB option" where
-"tsMedRSAbb bst x \<equiv> ((tsbDom\<cdot>x = {ar})
-                           \<leadsto> [as \<mapsto> (tsMap::(bool \<Rightarrow> 'a MABP) \<Rightarrow> bool tstream \<rightarrow> 'a MABP tstream) Bool\<cdot>(tsMed\<cdot>(tsMap invBool\<cdot>(x . ar))\<cdot>bst)]\<Omega>)"
+abbreviation tsMedRSAbb  :: "bool stream \<Rightarrow> 'a MABP tstream\<^sup>\<Omega> \<Rightarrow> ('a MABP tstream\<^sup>\<Omega>) option" where
+"tsMedRSAbb bst x \<equiv> ((ubclDom\<cdot>x = {c_ar})
+                            \<leadsto> Abs_ubundle([c_as \<mapsto> (tsMap::(bool \<Rightarrow> 'a MABP) \<Rightarrow> bool tstream \<rightarrow> 'a MABP tstream) Bool\<cdot>(tsMed\<cdot>(tsMap invBool\<cdot>(x . c_ar))\<cdot>bst)]))"
 
 subsection \<open>medium_sr\<close>
   (* medium from sender to receiver *)
-  (* input: ds, output: dr, transport (data, bool) tuples *)
+  (* input: c_ds, output: c_dr, transport (data, bool) tuples *)
 
-definition medSR_TSPF :: "bool stream \<Rightarrow> 'a MABP TSPF" where
-"medSR_TSPF bst\<equiv> Abs_CTSPF (\<lambda> x. (tsbDom\<cdot>x = {ds})
-  \<leadsto> [dr \<mapsto> (tsMap:: ('a \<times> bool \<Rightarrow> 'a MABP) \<Rightarrow> ('a \<times> bool) tstream \<rightarrow> 'a MABP tstream) 
-            BoolPair\<cdot>(tsMed\<cdot>(tsMap invBoolPair\<cdot>(x . ds))\<cdot>bst)]\<Omega>)"
+definition medSR_TSPF :: "bool stream \<Rightarrow> ('a MABP tstream\<^sup>\<Omega>, 'a MABP tstream\<^sup>\<Omega>) ufun" where
+"medSR_TSPF bst\<equiv> Abs_cufun (\<lambda> x. (ubclDom\<cdot>x = {c_ds})
+  \<leadsto> Abs_ubundle([c_dr \<mapsto> (tsMap:: ('a \<times> bool \<Rightarrow> 'a MABP) \<Rightarrow> ('a \<times> bool) tstream \<rightarrow> 'a MABP tstream) 
+            BoolPair\<cdot>(tsMed\<cdot>(tsMap invBoolPair\<cdot>(x . c_ds))\<cdot>bst)]))"
 
-abbreviation medSR_TSPFAbb  :: "bool stream \<Rightarrow> 'a MABP TSB \<Rightarrow> 'a MABP TSB option" where
-"medSR_TSPFAbb bst x \<equiv> ((tsbDom\<cdot>x = {ds})
-  \<leadsto> [dr \<mapsto> (tsMap:: ('a \<times> bool \<Rightarrow> 'a MABP) \<Rightarrow> ('a \<times> bool) tstream \<rightarrow> 'a MABP tstream) 
-            BoolPair\<cdot>(tsMed\<cdot>(tsMap invBoolPair\<cdot>(x . ds))\<cdot>bst)]\<Omega>)"
+abbreviation medSR_TSPFAbb  :: "bool stream \<Rightarrow> 'a MABP tstream\<^sup>\<Omega> \<Rightarrow> ('a MABP tstream\<^sup>\<Omega>) option" where
+"medSR_TSPFAbb bst x \<equiv> ((ubclDom\<cdot>x = {c_ds})
+  \<leadsto> Abs_ubundle([c_dr \<mapsto> (tsMap:: ('a \<times> bool \<Rightarrow> 'a MABP) \<Rightarrow> ('a \<times> bool) tstream \<rightarrow> 'a MABP tstream) 
+            BoolPair\<cdot>(tsMed\<cdot>(tsMap invBoolPair\<cdot>(x . c_ds))\<cdot>bst)]))"
 
 subsection \<open>sender\<close>
 
   (* lift a sender function to a TSPF *)
-definition sender_TSPF :: "'a sender \<Rightarrow> 'a MABP TSPF" where
-"sender_TSPF se \<equiv> Abs_CTSPF (\<lambda> x. (tsbDom\<cdot>x = {as, abpIn})
-                \<leadsto> [ds \<mapsto> tsMap BoolPair\<cdot>(se\<cdot>(tsMap invData\<cdot>(x . abpIn))\<cdot>(tsMap invBool\<cdot>(x . as)))]\<Omega>)"
+definition sender_TSPF :: "'a sender \<Rightarrow> ('a MABP tstream\<^sup>\<Omega>, 'a MABP tstream\<^sup>\<Omega>) ufun" where
+"sender_TSPF se \<equiv> Abs_cufun (\<lambda> x. (ubclDom\<cdot>x = {c_as, c_abpIn})
+                \<leadsto> Abs_ubundle([c_ds \<mapsto> tsMap BoolPair\<cdot>(se\<cdot>(tsMap invData\<cdot>(x . c_abpIn))\<cdot>(tsMap invBool\<cdot>(x . c_as)))]))"
 
-*)
+
 (* ----------------------------------------------------------------------- *)
 section \<open>lemmata\<close>
 (* ----------------------------------------------------------------------- *)
@@ -137,10 +137,10 @@ subsubsection \<open>defs\<close>
 
       (* helper functions to prove cont *)
 definition recvCH1 :: "'a MABP tstream\<^sup>\<Omega> \<Rightarrow> 'a MABP tstream"  where
-"recvCH1 \<equiv> (\<lambda> x. tsMap Bool\<cdot>(fst (tsRec\<cdot>((tsMap invBoolPair)\<cdot>(x .dr)))))"
+"recvCH1 \<equiv> (\<lambda> x. tsMap Bool\<cdot>(fst (tsRec\<cdot>((tsMap invBoolPair)\<cdot>(x .c_dr)))))"
 
 definition recvCH2 :: "'a MABP tstream\<^sup>\<Omega> \<Rightarrow> 'a MABP tstream"  where
-"recvCH2 \<equiv> (\<lambda> x. tsMap Data\<cdot>(snd (tsRec\<cdot>((tsMap invBoolPair)\<cdot>(x .dr)))))"
+"recvCH2 \<equiv> (\<lambda> x. tsMap Data\<cdot>(snd (tsRec\<cdot>((tsMap invBoolPair)\<cdot>(x .c_dr)))))"
 
 lemma recvCH1_contlub: assumes "chain Y"
   shows "recvCH1 ((\<Squnion>i. Y i)) = (\<Squnion>i. (recvCH1 ((Y i))))"
@@ -152,208 +152,175 @@ lemma recvCH2_contlub: assumes "chain Y"
   apply (rule cont2contlubE)
   by (simp_all add: assms recvCH2_def)
 
-lemma to_recvch1: "tsMap Bool\<cdot>(fst (tsRec\<cdot>((tsMap invBoolPair)\<cdot>(x .dr))))
+lemma to_recvch1: "tsMap Bool\<cdot>(fst (tsRec\<cdot>((tsMap invBoolPair)\<cdot>(x .c_dr))))
                     = (recvCH1::'a MABP tstream\<^sup>\<Omega> \<Rightarrow> 'a MABP tstream) x"
   by (simp add: recvCH1_def)
 
-lemma to_recvch2: "tsMap Data\<cdot>(snd (tsRec\<cdot>((tsMap invBoolPair)\<cdot>(x .dr))))
+lemma to_recvch2: "tsMap Data\<cdot>(snd (tsRec\<cdot>((tsMap invBoolPair)\<cdot>(x .c_dr))))
                     = (recvCH2::'a MABP tstream\<^sup>\<Omega> \<Rightarrow> 'a MABP tstream) x"
   by (simp add: recvCH2_def)
 
 lemma recv_tsb_well [simp]:
-  shows "ubWell [ar \<mapsto> tsMap Bool\<cdot>(fst (tsRec\<cdot>((tsMap invBoolPair)\<cdot>(x . dr)))),
-                                  abpOut \<mapsto> tsMap Data\<cdot>(snd (tsRec\<cdot>((tsMap invBoolPair)\<cdot>(x . dr))))]"
+  shows "ubWell [c_ar \<mapsto> tsMap Bool\<cdot>(fst (tsRec\<cdot>((tsMap invBoolPair)\<cdot>(x . c_dr)))),
+                                  c_abpOut \<mapsto> tsMap Data\<cdot>(snd (tsRec\<cdot>((tsMap invBoolPair)\<cdot>(x . c_dr))))]"
   apply (rule ubwellI)
   apply (simp add: tsmap_tsdom_range)
-  by (metis ctype_MABP.simps(2) ctype_MABP.simps(6) tsmap_tsdom_range usOkay_tstream_def)
+  by (metis ctype_MABP.simps(2) ctype_MABP.simps(6) tsmap_tsdom_range usclOkay_tstream_def)
 
-lemma recv_tsb_dom: "ubDom\<cdot>(Abs_ubundle([ar \<mapsto> tsMap Bool\<cdot>(fst (tsRec\<cdot>((tsMap invBoolPair)\<cdot>(x . dr)))),
-                              abpOut \<mapsto> tsMap Data\<cdot>(snd (tsRec\<cdot>((tsMap invBoolPair)\<cdot>(x . dr))))]))
-                     = {ar, abpOut}"
-  apply (simp add: ubdom_ubrep_eq)
-    by auto
-
+lemma recv_tsb_dom: "ubclDom\<cdot>(Abs_ubundle([c_ar \<mapsto> tsMap Bool\<cdot>(fst (tsRec\<cdot>((tsMap invBoolPair)\<cdot>(x . c_dr)))),
+                              c_abpOut \<mapsto> tsMap Data\<cdot>(snd (tsRec\<cdot>((tsMap invBoolPair)\<cdot>(x . c_dr))))]))
+                     = {c_ar, c_abpOut}"
+  by (simp add: insert_commute ubclDom_ubundle_def ubdom_ubrep_eq)
 
 
-lemma rec_tsb_mono: "\<And>(x::'a MABP tstream ubundle) y::'a MABP tstream ubundle. ubDom\<cdot>x = {dr} \<Longrightarrow> x \<sqsubseteq> y \<Longrightarrow>
-          Abs_ubundle([ar \<mapsto> tsMap Bool\<cdot>(fst (tsRec\<cdot>(tsMap invBoolPair\<cdot>(x  .  dr)))),
-          abpOut \<mapsto> tsMap Data\<cdot>(snd (tsRec\<cdot>(tsMap invBoolPair\<cdot>(x  .  dr))))])
-          \<sqsubseteq> Abs_ubundle([ar \<mapsto> tsMap Bool\<cdot>(fst (tsRec\<cdot>(tsMap invBoolPair\<cdot>(y  .  dr)))),
-             abpOut \<mapsto> tsMap Data\<cdot>(snd (tsRec\<cdot>(tsMap invBoolPair\<cdot>(y  .  dr))))])"
+
+lemma rec_tsb_mono: "\<And>(x::'a MABP tstream ubundle) y::'a MABP tstream ubundle. ubclDom\<cdot>x = {c_dr} \<Longrightarrow> x \<sqsubseteq> y \<Longrightarrow>
+          Abs_ubundle([c_ar \<mapsto> tsMap Bool\<cdot>(fst (tsRec\<cdot>(tsMap invBoolPair\<cdot>(x  .  c_dr)))),
+          c_abpOut \<mapsto> tsMap Data\<cdot>(snd (tsRec\<cdot>(tsMap invBoolPair\<cdot>(x  .  c_dr))))])
+          \<sqsubseteq> Abs_ubundle([c_ar \<mapsto> tsMap Bool\<cdot>(fst (tsRec\<cdot>(tsMap invBoolPair\<cdot>(y  .  c_dr)))),
+             c_abpOut \<mapsto> tsMap Data\<cdot>(snd (tsRec\<cdot>(tsMap invBoolPair\<cdot>(y  .  c_dr))))])"
       apply (rule ub_below)
        apply (simp_all add: ubdom_below ubdom_ubrep_eq ubgetch_ubrep_eq)
        by (simp add: fst_monofun snd_monofun monofun_cfun_arg ubgetch_below)
 
 
-lemma recvTSPF_mono [simp]: "monofun (\<lambda> x. (ubDom\<cdot>x = {dr}) \<leadsto>
-                                    Abs_ubundle([ar \<mapsto> tsMap Bool\<cdot>(fst (tsRec\<cdot>((tsMap invBoolPair)\<cdot>(x . dr)))),
-                                     abpOut \<mapsto> tsMap Data\<cdot>(snd (tsRec\<cdot>((tsMap invBoolPair)\<cdot>(x . dr))))]))"
-  apply (simp add: monofun_def)
-  apply (simp add: rec_tsb_mono some_below ubdom_below)
-  using ubdom_below by auto
+lemma recvTSPF_mono [simp]: "monofun (\<lambda> x. (ubclDom\<cdot>x = {c_dr}) \<leadsto>
+                                    Abs_ubundle([c_ar \<mapsto> tsMap Bool\<cdot>(fst (tsRec\<cdot>((tsMap invBoolPair)\<cdot>(x . c_dr)))),
+                                     c_abpOut \<mapsto> tsMap Data\<cdot>(snd (tsRec\<cdot>((tsMap invBoolPair)\<cdot>(x . c_dr))))]))"
+  apply (rule monofunI)
+  apply (case_tac "ubclDom\<cdot>x = {c_dr}")
+   apply (simp add: ubdom_below rec_tsb_mono some_below ubcldom_fix)
+  by (simp add: ubdom_below ubcldom_fix)
 
-lemma recvTSPF_tsb_getc: assumes "chain Y" and "ubDom\<cdot>(\<Squnion>i. Y i) = {dr}"
-  and "c \<in>  {ar, abpOut}"
+lemma recvTSPF_tsb_getc: assumes "chain Y" and "ubclDom\<cdot>(\<Squnion>i. Y i) = {c_dr}"
+  and "c \<in>  {c_ar, c_abpOut}"
   shows " (\<Squnion>i.
-           Abs_ubundle([ar \<mapsto> tsMap Bool\<cdot>(fst (tsRec\<cdot>(tsMap invBoolPair\<cdot>(Y i  .  dr)))), abpOut \<mapsto>
-            tsMap Data\<cdot>(snd (tsRec\<cdot>(tsMap invBoolPair\<cdot>(Y i  .  dr))))])) . c
-          = (\<Squnion> i. (Abs_ubundle([ar \<mapsto> tsMap Bool\<cdot>(fst (tsRec\<cdot>(tsMap invBoolPair\<cdot>(Y i  .  dr)))), abpOut \<mapsto>
-            tsMap Data\<cdot>(snd (tsRec\<cdot>(tsMap invBoolPair\<cdot>(Y i  .  dr))))])) . c)"
+           Abs_ubundle([c_ar \<mapsto> tsMap Bool\<cdot>(fst (tsRec\<cdot>(tsMap invBoolPair\<cdot>(Y i  .  c_dr)))), c_abpOut \<mapsto>
+            tsMap Data\<cdot>(snd (tsRec\<cdot>(tsMap invBoolPair\<cdot>(Y i  .  c_dr))))])) . c
+          = (\<Squnion> i. (Abs_ubundle([c_ar \<mapsto> tsMap Bool\<cdot>(fst (tsRec\<cdot>(tsMap invBoolPair\<cdot>(Y i  .  c_dr)))), c_abpOut \<mapsto>
+            tsMap Data\<cdot>(snd (tsRec\<cdot>(tsMap invBoolPair\<cdot>(Y i  .  c_dr))))])) . c)"
 proof (rule lubgetCh)
-   have f2: "\<And> i. ubDom\<cdot>(Y i) =  ubDom\<cdot>(\<Squnion>i. Y i)"
-     by (simp add: assms(1))
-   show tb_chain: "chain (\<lambda>i::nat. Abs_ubundle([ar \<mapsto> tsMap Bool\<cdot>(fst (tsRec\<cdot>(tsMap invBoolPair\<cdot>(Y i  .  dr)))),
-                             abpOut \<mapsto> tsMap Data\<cdot>(snd (tsRec\<cdot>(tsMap invBoolPair\<cdot>(Y i  .  dr))))]))"
-     by (simp add: assms(1) assms(2) po_class.chainE po_class.chainI rec_tsb_mono)
+   have f2: "\<And> i. ubclDom\<cdot>(Y i) =  ubclDom\<cdot>(\<Squnion>i. Y i)"
+     by (simp add: assms(1) ubclDom_ubundle_def)
+   show tb_chain: "chain (\<lambda>i::nat. Abs_ubundle([c_ar \<mapsto> tsMap Bool\<cdot>(fst (tsRec\<cdot>(tsMap invBoolPair\<cdot>(Y i  .  c_dr)))),
+                             c_abpOut \<mapsto> tsMap Data\<cdot>(snd (tsRec\<cdot>(tsMap invBoolPair\<cdot>(Y i  .  c_dr))))]))"
+     by (simp add: assms(1) assms(2) f2 po_class.chainE po_class.chainI rec_tsb_mono)
 
-   show " c \<in> ubDom\<cdot>(\<Squnion>i::nat.
-                          Abs_ubundle([ar \<mapsto> tsMap Bool\<cdot>(fst (tsRec\<cdot>(tsMap invBoolPair\<cdot>(Y i  .  dr)))),
-                       abpOut \<mapsto> tsMap Data\<cdot>(snd (tsRec\<cdot>(tsMap invBoolPair\<cdot>(Y i  .  dr))))]))"
-     using assms(3) recv_tsb_dom tb_chain ubdom_chain_eq2 by blast
+   show " c \<in> ubclDom\<cdot>(\<Squnion>i::nat.
+                          Abs_ubundle([c_ar \<mapsto> tsMap Bool\<cdot>(fst (tsRec\<cdot>(tsMap invBoolPair\<cdot>(Y i  .  c_dr)))),
+                       c_abpOut \<mapsto> tsMap Data\<cdot>(snd (tsRec\<cdot>(tsMap invBoolPair\<cdot>(Y i  .  c_dr))))]))"
+     using assms(3) recv_tsb_dom tb_chain ubcldom_lub_eq2I by blast
 qed
 
 
   (* show that recTSPF is cont, proof concept taken from TSPF_Template_CaseStudy *)
 lemma recvTSPF_cont [simp]:
-  shows "cont (\<lambda> x. (ubDom\<cdot>x = {dr}) \<leadsto>
-                      Abs_ubundle([ar \<mapsto> (tsMap::(bool \<Rightarrow> 'a MABP) \<Rightarrow> bool tstream \<rightarrow> 'a MABP tstream)
+  shows "cont (\<lambda> x. (ubclDom\<cdot>x = {c_dr}) \<leadsto>
+                      Abs_ubundle([c_ar \<mapsto> (tsMap::(bool \<Rightarrow> 'a MABP) \<Rightarrow> bool tstream \<rightarrow> 'a MABP tstream)
                             Bool\<cdot>(fst ((tsRec::('a * bool) tstream \<rightarrow> (bool tstream \<times> 'a tstream))\<cdot>
-                            ((tsMap invBoolPair)\<cdot>(x . dr)))),
-                       abpOut \<mapsto> (tsMap::('a \<Rightarrow> 'a MABP) \<Rightarrow> 'a tstream \<rightarrow> 'a MABP tstream)
-                            Data\<cdot>(snd (tsRec\<cdot>((tsMap invBoolPair)\<cdot>(x . dr))))]))"
-proof (rule contI2)
-  show "monofun (\<lambda>x::'a MABP tstream\<^sup>\<Omega>. (UBundle.ubDom\<cdot>x = {dr})\<leadsto>
-          Abs_ubundle [ar \<mapsto> tsMap Bool\<cdot>(fst (tsRec\<cdot>(tsMap invBoolPair\<cdot>(x  .  dr)))), 
-            abpOut \<mapsto> tsMap Data\<cdot>(snd (tsRec\<cdot>(tsMap invBoolPair\<cdot>(x  .  dr))))])"
-    by simp
-next
-  show "\<forall>Y::nat \<Rightarrow> 'a MABP tstream\<^sup>\<Omega>.
-       chain Y \<longrightarrow>
-       (UBundle.ubDom\<cdot>(\<Squnion>i::nat. Y i) =
-        {dr})\<leadsto>Abs_ubundle [ar \<mapsto> tsMap Bool\<cdot>(fst (tsRec\<cdot>(tsMap invBoolPair\<cdot>((\<Squnion>i::nat. Y i)  .  dr)))), abpOut \<mapsto> tsMap Data\<cdot>(snd (tsRec\<cdot>(tsMap invBoolPair\<cdot>((\<Squnion>i::nat. Y i)  .  dr))))] \<sqsubseteq>
-       (\<Squnion>i::nat. (UBundle.ubDom\<cdot>(Y i) = {dr})\<leadsto>Abs_ubundle [ar \<mapsto> tsMap Bool\<cdot>(fst (tsRec\<cdot>(tsMap invBoolPair\<cdot>(Y i  .  dr)))), abpOut \<mapsto> tsMap Data\<cdot>(snd (tsRec\<cdot>(tsMap invBoolPair\<cdot>(Y i  .  dr))))])"
-  proof (rule allI, rule impI)
+                            ((tsMap invBoolPair)\<cdot>(x . c_dr)))),
+                       c_abpOut \<mapsto> (tsMap::('a \<Rightarrow> 'a MABP) \<Rightarrow> 'a tstream \<rightarrow> 'a MABP tstream)
+                            Data\<cdot>(snd (tsRec\<cdot>((tsMap invBoolPair)\<cdot>(x . c_dr))))]))"
+proof (rule ufun_contI, simp add: rec_tsb_mono)
     fix Y::"nat \<Rightarrow> 'a MABP tstream\<^sup>\<Omega>"
-    assume Y_is_chain: "chain Y"
-    have f1: "(ubDom\<cdot>(\<Squnion>i. Y i)) = (\<Squnion>i. (UBundle.ubDom\<cdot>(Y i)))"
-      using Y_is_chain by auto
-    show "(UBundle.ubDom\<cdot>(\<Squnion>i::nat. Y i) =
-        {dr})\<leadsto>Abs_ubundle [ar \<mapsto> tsMap Bool\<cdot>(fst (tsRec\<cdot>(tsMap invBoolPair\<cdot>((\<Squnion>i::nat. Y i)  .  dr)))), abpOut \<mapsto> tsMap Data\<cdot>(snd (tsRec\<cdot>(tsMap invBoolPair\<cdot>((\<Squnion>i::nat. Y i)  .  dr))))] \<sqsubseteq>
-       (\<Squnion>i::nat. (UBundle.ubDom\<cdot>(Y i) = {dr})\<leadsto>Abs_ubundle [ar \<mapsto> tsMap Bool\<cdot>(fst (tsRec\<cdot>(tsMap invBoolPair\<cdot>(Y i  .  dr)))), abpOut \<mapsto> tsMap Data\<cdot>(snd (tsRec\<cdot>(tsMap invBoolPair\<cdot>(Y i  .  dr))))])"
-    proof (cases "ubDom\<cdot>(\<Squnion>i::nat. Y i) = {dr}")
-      case True
-      have f11: "\<And>i . (UBundle.ubDom\<cdot>(Y i)) = {dr}"
-        by (simp add: True Y_is_chain)
-      have f12: "(UBundle.ubDom\<cdot>(\<Squnion>i::nat. Y i) =
-        {dr})\<leadsto>Abs_ubundle [ar \<mapsto> tsMap Bool\<cdot>(fst (tsRec\<cdot>(tsMap invBoolPair\<cdot>((\<Squnion>i::nat. Y i)  .  dr)))), abpOut \<mapsto> tsMap Data\<cdot>(snd (tsRec\<cdot>(tsMap invBoolPair\<cdot>((\<Squnion>i::nat. Y i)  .  dr))))] = 
-            Some (Abs_ubundle [ar \<mapsto> tsMap Bool\<cdot>(fst (tsRec\<cdot>(tsMap invBoolPair\<cdot>((\<Squnion>i::nat. Y i)  .  dr)))), abpOut \<mapsto> tsMap Data\<cdot>(snd (tsRec\<cdot>(tsMap invBoolPair\<cdot>((\<Squnion>i::nat. Y i)  .  dr))))])"
-        by (simp add: True)
-      have f13: "(\<Squnion>i::nat. (UBundle.ubDom\<cdot>(Y i) = {dr})\<leadsto>Abs_ubundle [ar \<mapsto> tsMap Bool\<cdot>(fst (tsRec\<cdot>(tsMap invBoolPair\<cdot>(Y i  .  dr)))), abpOut \<mapsto> tsMap Data\<cdot>(snd (tsRec\<cdot>(tsMap invBoolPair\<cdot>(Y i  .  dr))))]) = 
-            (\<Squnion>i::nat. Some (Abs_ubundle [ar \<mapsto> tsMap Bool\<cdot>(fst (tsRec\<cdot>(tsMap invBoolPair\<cdot>(Y i  .  dr)))), abpOut \<mapsto> tsMap Data\<cdot>(snd (tsRec\<cdot>(tsMap invBoolPair\<cdot>(Y i  .  dr))))]))"
-        by (simp add: f11)
-      have f14:"Some (\<Squnion>i::nat. (Abs_ubundle [ar \<mapsto> tsMap Bool\<cdot>(fst (tsRec\<cdot>(tsMap invBoolPair\<cdot>(Y i  .  dr)))), abpOut \<mapsto> tsMap Data\<cdot>(snd (tsRec\<cdot>(tsMap invBoolPair\<cdot>(Y i  .  dr))))]))
-          = (\<Squnion>i::nat. Some (Abs_ubundle [ar \<mapsto> tsMap Bool\<cdot>(fst (tsRec\<cdot>(tsMap invBoolPair\<cdot>(Y i  .  dr)))), abpOut \<mapsto> tsMap Data\<cdot>(snd (tsRec\<cdot>(tsMap invBoolPair\<cdot>(Y i  .  dr))))]))"
-        apply (rule some_lub_chain_eq)
-        apply (simp add: chain_def)
-        by (simp add: Y_is_chain f11 po_class.chainE rec_tsb_mono)
-      have f15: "UBundle.ubDom\<cdot>(Abs_ubundle [ar \<mapsto> tsMap Bool\<cdot>(fst (tsRec\<cdot>(tsMap invBoolPair\<cdot>((\<Squnion>i::nat. Y i)  .  dr)))), abpOut \<mapsto> tsMap Data\<cdot>(snd (tsRec\<cdot>(tsMap invBoolPair\<cdot>((\<Squnion>i::nat. Y i)  .  dr))))]) = 
-                ubDom\<cdot>(\<Squnion>i::nat. (Abs_ubundle [ar \<mapsto> tsMap Bool\<cdot>(fst (tsRec\<cdot>(tsMap invBoolPair\<cdot>(Y i  .  dr)))), abpOut \<mapsto> tsMap Data\<cdot>(snd (tsRec\<cdot>(tsMap invBoolPair\<cdot>(Y i  .  dr))))]))"
-        by (metis (mono_tags, lifting) Y_is_chain f11 po_class.chain_def rec_tsb_mono recv_tsb_dom ubdom_chain_eq2)
-      have f17: "\<And> c::channel. (\<Squnion>i::nat. Abs_ubundle [ar \<mapsto> tsMap Bool\<cdot>(fst (tsRec\<cdot>(tsMap invBoolPair\<cdot>(Y i  .  dr)))), abpOut \<mapsto> tsMap Data\<cdot>(snd (tsRec\<cdot>(tsMap invBoolPair\<cdot>(Y i  .  dr))))])  .  c = 
-          (\<Squnion>i::nat. Abs_ubundle [ar \<mapsto> tsMap Bool\<cdot>(fst (tsRec\<cdot>(tsMap invBoolPair\<cdot>(Y i  .  dr)))), abpOut \<mapsto> tsMap Data\<cdot>(snd (tsRec\<cdot>(tsMap invBoolPair\<cdot>(Y i  .  dr))))] . c)"
-        apply (rule cont2contlubE)
-        by (simp add: Y_is_chain f11 po_class.chainE po_class.chainI rec_tsb_mono) +
-      have f16: "\<And>c::channel.
-       c \<in> UBundle.ubDom\<cdot>(Abs_ubundle [ar \<mapsto> tsMap Bool\<cdot>(fst (tsRec\<cdot>(tsMap invBoolPair\<cdot>((\<Squnion>i::nat. Y i)  .  dr)))), abpOut \<mapsto> tsMap Data\<cdot>(snd (tsRec\<cdot>(tsMap invBoolPair\<cdot>((\<Squnion>i::nat. Y i)  .  dr))))]) \<Longrightarrow>
-       Abs_ubundle [ar \<mapsto> tsMap Bool\<cdot>(fst (tsRec\<cdot>(tsMap invBoolPair\<cdot>((\<Squnion>i::nat. Y i)  .  dr)))), abpOut \<mapsto> tsMap Data\<cdot>(snd (tsRec\<cdot>(tsMap invBoolPair\<cdot>((\<Squnion>i::nat. Y i)  .  dr))))]  .  c \<sqsubseteq>
-       (\<Squnion>i::nat. Abs_ubundle [ar \<mapsto> tsMap Bool\<cdot>(fst (tsRec\<cdot>(tsMap invBoolPair\<cdot>(Y i  .  dr)))), abpOut \<mapsto> tsMap Data\<cdot>(snd (tsRec\<cdot>(tsMap invBoolPair\<cdot>(Y i  .  dr))))])  .  c"
-      proof -
-        fix c::channel
-        assume "c \<in> UBundle.ubDom\<cdot>(Abs_ubundle [ar \<mapsto> tsMap Bool\<cdot>(fst (tsRec\<cdot>(tsMap invBoolPair\<cdot>((\<Squnion>i::nat. Y i)  .  dr)))), abpOut \<mapsto> tsMap Data\<cdot>(snd (tsRec\<cdot>(tsMap invBoolPair\<cdot>((\<Squnion>i::nat. Y i)  .  dr))))])"
-        then have f160: "c \<in>  {ar, abpOut}"
-          by (simp add: recv_tsb_dom)
-        show "Abs_ubundle [ar \<mapsto> tsMap Bool\<cdot>(fst (tsRec\<cdot>(tsMap invBoolPair\<cdot>((\<Squnion>i::nat. Y i)  .  dr)))), abpOut \<mapsto> tsMap Data\<cdot>(snd (tsRec\<cdot>(tsMap invBoolPair\<cdot>((\<Squnion>i::nat. Y i)  .  dr))))]  .  c \<sqsubseteq>
-       (\<Squnion>i::nat. Abs_ubundle [ar \<mapsto> tsMap Bool\<cdot>(fst (tsRec\<cdot>(tsMap invBoolPair\<cdot>(Y i  .  dr)))), abpOut \<mapsto> tsMap Data\<cdot>(snd (tsRec\<cdot>(tsMap invBoolPair\<cdot>(Y i  .  dr))))])  .  c"
-          apply (subst f17)
-          apply (simp add: recvTSPF_tsb_getc ubdom_ubrep_eq ubgetch_ubrep_eq)
-          apply (rule conjI)
-           apply (metis (mono_tags, lifting) Y_is_chain eq_imp_below lub_eq recvCH1_contlub to_recvch1)
-          by (simp add: Y_is_chain recvCH2_contlub to_recvch2)
-      qed
-      have f20: "Some (Abs_ubundle [ar \<mapsto> tsMap Bool\<cdot>(fst (tsRec\<cdot>(tsMap invBoolPair\<cdot>((\<Squnion>i::nat. Y i)  .  dr)))), abpOut \<mapsto> tsMap Data\<cdot>(snd (tsRec\<cdot>(tsMap invBoolPair\<cdot>((\<Squnion>i::nat. Y i)  .  dr))))]) \<sqsubseteq>
-       Some (\<Squnion>i::nat. (Abs_ubundle [ar \<mapsto> tsMap Bool\<cdot>(fst (tsRec\<cdot>(tsMap invBoolPair\<cdot>(Y i  .  dr)))), abpOut \<mapsto> tsMap Data\<cdot>(snd (tsRec\<cdot>(tsMap invBoolPair\<cdot>(Y i  .  dr))))]))"
-        apply (rule some_below)
-        apply (rule ub_below)
-         apply (metis (mono_tags, lifting) Y_is_chain f11 po_class.chain_def rec_tsb_mono recv_tsb_dom ubdom_chain_eq2)
-        by (simp add: f16)
-      then show ?thesis 
-        using True f13 f14 by auto
-    next
-      case False
-      then show ?thesis
-        using Y_is_chain by auto 
-    qed
-  qed
+    assume Y_is_chain: "chain Y" and chain_Y_dom: "ubclDom\<cdot>(\<Squnion>i::nat. Y i) = {c_dr}"
+    have f1: "\<And> i. (ubclDom\<cdot>(\<Squnion>i. Y i)) =  (ubclDom\<cdot>(Y i))"
+      by (simp add: Y_is_chain ubclDom_ubundle_def)
+    have f11: "\<And>i . (ubclDom\<cdot>(Y i)) = {c_dr}"
+      using chain_Y_dom f1 by auto
+    have "\<And> i. ubWell [c_ar \<mapsto> tsMap Bool\<cdot>(fst (tsRec\<cdot>(tsMap invBoolPair\<cdot>(Y i  .  c_dr)))), c_abpOut \<mapsto> tsMap Data\<cdot>(snd (tsRec\<cdot>(tsMap invBoolPair\<cdot>(Y i  .  c_dr))))]"
+      by simp
+    have f12: "(ubclDom\<cdot>(\<Squnion>i::nat. Y i) =
+        {c_dr})\<leadsto>Abs_ubundle [c_ar \<mapsto> tsMap Bool\<cdot>(fst (tsRec\<cdot>(tsMap invBoolPair\<cdot>((\<Squnion>i::nat. Y i)  .  c_dr)))), c_abpOut \<mapsto> tsMap Data\<cdot>(snd (tsRec\<cdot>(tsMap invBoolPair\<cdot>((\<Squnion>i::nat. Y i)  .  c_dr))))] = 
+            Some (Abs_ubundle [c_ar \<mapsto> tsMap Bool\<cdot>(fst (tsRec\<cdot>(tsMap invBoolPair\<cdot>((\<Squnion>i::nat. Y i)  .  c_dr)))), c_abpOut \<mapsto> tsMap Data\<cdot>(snd (tsRec\<cdot>(tsMap invBoolPair\<cdot>((\<Squnion>i::nat. Y i)  .  c_dr))))])"
+      by (simp add: chain_Y_dom)
+    have f13: "(\<Squnion>i::nat. (ubclDom\<cdot>(Y i) = {c_dr})\<leadsto>Abs_ubundle [c_ar \<mapsto> tsMap Bool\<cdot>(fst (tsRec\<cdot>(tsMap invBoolPair\<cdot>(Y i  .  c_dr)))), c_abpOut \<mapsto> tsMap Data\<cdot>(snd (tsRec\<cdot>(tsMap invBoolPair\<cdot>(Y i  .  c_dr))))]) = 
+            (\<Squnion>i::nat. Some (Abs_ubundle [c_ar \<mapsto> tsMap Bool\<cdot>(fst (tsRec\<cdot>(tsMap invBoolPair\<cdot>(Y i  .  c_dr)))), c_abpOut \<mapsto> tsMap Data\<cdot>(snd (tsRec\<cdot>(tsMap invBoolPair\<cdot>(Y i  .  c_dr))))]))"
+      by (simp add: f11)
+    have f14:"Some (\<Squnion>i::nat. (Abs_ubundle [c_ar \<mapsto> tsMap Bool\<cdot>(fst (tsRec\<cdot>(tsMap invBoolPair\<cdot>(Y i  .  c_dr)))), c_abpOut \<mapsto> tsMap Data\<cdot>(snd (tsRec\<cdot>(tsMap invBoolPair\<cdot>(Y i  .  c_dr))))]))
+          = (\<Squnion>i::nat. Some (Abs_ubundle [c_ar \<mapsto> tsMap Bool\<cdot>(fst (tsRec\<cdot>(tsMap invBoolPair\<cdot>(Y i  .  c_dr)))), c_abpOut \<mapsto> tsMap Data\<cdot>(snd (tsRec\<cdot>(tsMap invBoolPair\<cdot>(Y i  .  c_dr))))]))"
+      apply (rule some_lub_chain_eq)
+      apply (simp add: chain_def)
+      by (simp add: Y_is_chain f11 po_class.chainE rec_tsb_mono)
+    have f15: "ubclDom\<cdot>(Abs_ubundle [c_ar \<mapsto> tsMap Bool\<cdot>(fst (tsRec\<cdot>(tsMap invBoolPair\<cdot>((\<Squnion>i::nat. Y i)  .  c_dr)))), c_abpOut \<mapsto> tsMap Data\<cdot>(snd (tsRec\<cdot>(tsMap invBoolPair\<cdot>((\<Squnion>i::nat. Y i)  .  c_dr))))]) =
+                ubclDom\<cdot>(\<Squnion>i::nat. (Abs_ubundle [c_ar \<mapsto> tsMap Bool\<cdot>(fst (tsRec\<cdot>(tsMap invBoolPair\<cdot>(Y i  .  c_dr)))), c_abpOut \<mapsto> tsMap Data\<cdot>(snd (tsRec\<cdot>(tsMap invBoolPair\<cdot>(Y i  .  c_dr))))]))"
+      apply (simp add: ubclDom_ubundle_def)
+      by (metis (mono_tags, lifting) Y_is_chain f11 po_class.chain_def rec_tsb_mono recv_tsb_dom ubclDom_ubundle_def ubdom_chain_eq2)
+    have f17: "\<And> c::channel. (\<Squnion>i::nat. Abs_ubundle [c_ar \<mapsto> tsMap Bool\<cdot>(fst (tsRec\<cdot>(tsMap invBoolPair\<cdot>(Y i  .  c_dr)))), c_abpOut \<mapsto> tsMap Data\<cdot>(snd (tsRec\<cdot>(tsMap invBoolPair\<cdot>(Y i  .  c_dr))))])  .  c =
+          (\<Squnion>i::nat. Abs_ubundle [c_ar \<mapsto> tsMap Bool\<cdot>(fst (tsRec\<cdot>(tsMap invBoolPair\<cdot>(Y i  .  c_dr)))), c_abpOut \<mapsto> tsMap Data\<cdot>(snd (tsRec\<cdot>(tsMap invBoolPair\<cdot>(Y i  .  c_dr))))] . c)"
+      apply (rule cont2contlubE)
+      by (simp add: Y_is_chain f11 po_class.chainE po_class.chainI rec_tsb_mono) +
+    have f20: "Some (Abs_ubundle [c_ar \<mapsto> tsMap Bool\<cdot>(fst (tsRec\<cdot>(tsMap invBoolPair\<cdot>((\<Squnion>i::nat. Y i)  .  c_dr)))), c_abpOut \<mapsto> tsMap Data\<cdot>(snd (tsRec\<cdot>(tsMap invBoolPair\<cdot>((\<Squnion>i::nat. Y i)  .  c_dr))))]) \<sqsubseteq>
+       Some (\<Squnion>i::nat. (Abs_ubundle [c_ar \<mapsto> tsMap Bool\<cdot>(fst (tsRec\<cdot>(tsMap invBoolPair\<cdot>(Y i  .  c_dr)))), c_abpOut \<mapsto> tsMap Data\<cdot>(snd (tsRec\<cdot>(tsMap invBoolPair\<cdot>(Y i  .  c_dr))))]))"
+      apply (rule some_below)
+      apply (rule ub_below)
+       apply (metis (no_types, lifting) f15 ubclDom_ubundle_def)      
+      apply (subst f17)
+      apply (simp add: recvTSPF_tsb_getc ubdom_ubrep_eq ubgetch_ubrep_eq) 
+      by (metis (mono_tags, lifting) Y_is_chain eq_imp_below lub_eq recvCH1_contlub recvCH2_contlub to_recvch1 to_recvch2)
+    show "Abs_ubundle [c_ar \<mapsto> tsMap Bool\<cdot>(fst (tsRec\<cdot>(tsMap invBoolPair\<cdot>((\<Squnion>i::nat. Y i)  .  c_dr)))), c_abpOut \<mapsto> tsMap Data\<cdot>(snd (tsRec\<cdot>(tsMap invBoolPair\<cdot>((\<Squnion>i::nat. Y i)  .  c_dr))))] \<sqsubseteq>
+       (\<Squnion>i::nat. Abs_ubundle [c_ar \<mapsto> tsMap Bool\<cdot>(fst (tsRec\<cdot>(tsMap invBoolPair\<cdot>(Y i  .  c_dr)))), c_abpOut \<mapsto> tsMap Data\<cdot>(snd (tsRec\<cdot>(tsMap invBoolPair\<cdot>(Y i  .  c_dr))))])"
+      using f20 some_below2 by blast
 qed
 (* proof (rule ufun_contI)
-    show recv_mono: "\<And>(x::'a MABP tstream\<^sup>\<Omega>) y::'a MABP tstream\<^sup>\<Omega>. ubDom\<cdot>x = {dr} \<Longrightarrow> x \<sqsubseteq> y \<Longrightarrow>
-          Abs_ubundle([ar \<mapsto> tsMap Bool\<cdot>(fst (tsRec\<cdot>(tsMap invBoolPair\<cdot>(x  .  dr)))),
-          abpOut \<mapsto> tsMap Data\<cdot>(snd (tsRec\<cdot>(tsMap invBoolPair\<cdot>(x  .  dr))))])
-          \<sqsubseteq> Abs_ubundle([ar \<mapsto> tsMap Bool\<cdot>(fst (tsRec\<cdot>(tsMap invBoolPair\<cdot>(y  .  dr)))),
-             abpOut \<mapsto> tsMap Data\<cdot>(snd (tsRec\<cdot>(tsMap invBoolPair\<cdot>(y  .  dr))))])"
+    show recv_mono: "\<And>(x::'a MABP tstream\<^sup>\<Omega>) y::'a MABP tstream\<^sup>\<Omega>. ubclDom\<cdot>x = {c_dr} \<Longrightarrow> x \<sqsubseteq> y \<Longrightarrow>
+          Abs_ubundle([c_ar \<mapsto> tsMap Bool\<cdot>(fst (tsRec\<cdot>(tsMap invBoolPair\<cdot>(x  .  c_dr)))),
+          c_abpOut \<mapsto> tsMap Data\<cdot>(snd (tsRec\<cdot>(tsMap invBoolPair\<cdot>(x  .  c_dr))))])
+          \<sqsubseteq> Abs_ubundle([c_ar \<mapsto> tsMap Bool\<cdot>(fst (tsRec\<cdot>(tsMap invBoolPair\<cdot>(y  .  c_dr)))),
+             c_abpOut \<mapsto> tsMap Data\<cdot>(snd (tsRec\<cdot>(tsMap invBoolPair\<cdot>(y  .  c_dr))))])"
       by (simp add: rec_tsb_mono)
 
-    have f1: " \<And>Y::nat \<Rightarrow> 'a MABP tstream\<^sup>\<Omega>. chain Y \<Longrightarrow> ubDom\<cdot>(\<Squnion>i::nat. Y i) = {dr} \<Longrightarrow>
-                ubDom\<cdot>(\<Squnion>i::nat. Abs_ubundle([ar \<mapsto> tsMap Bool\<cdot>(fst (tsRec\<cdot>(tsMap invBoolPair\<cdot>(Y i  .  dr)))),
-                abpOut \<mapsto> tsMap Data\<cdot>(snd (tsRec\<cdot>(tsMap invBoolPair\<cdot>(Y i  .  dr))))])) = {abpOut, ar}"
+    have f1: " \<And>Y::nat \<Rightarrow> 'a MABP tstream\<^sup>\<Omega>. chain Y \<Longrightarrow> ubclDom\<cdot>(\<Squnion>i::nat. Y i) = {c_dr} \<Longrightarrow>
+                ubclDom\<cdot>(\<Squnion>i::nat. Abs_ubundle([c_ar \<mapsto> tsMap Bool\<cdot>(fst (tsRec\<cdot>(tsMap invBoolPair\<cdot>(Y i  .  c_dr)))),
+                c_abpOut \<mapsto> tsMap Data\<cdot>(snd (tsRec\<cdot>(tsMap invBoolPair\<cdot>(Y i  .  c_dr))))])) = {c_abpOut, c_ar}"
      proof -
       fix Y :: "nat \<Rightarrow> 'a MABP tstream\<^sup>\<Omega>"
       assume a1: "chain Y"
-      assume a2: "ubDom\<cdot>(\<Squnion>i. Y i) = {dr}"
-      have f3: "\<forall>t ta. (ubDom\<cdot>t \<noteq> {dr} \<or> t \<notsqsubseteq> ta)
-                        \<or> Abs_ubundle([ar \<mapsto> tsMap Bool\<cdot> (fst (tsRec\<cdot>(tsMap invBoolPair\<cdot>(t . dr)))),
-                            abpOut \<mapsto> tsMap Data\<cdot> (snd (tsRec\<cdot> (tsMap invBoolPair\<cdot> (t . dr)))::'a tstream)])
-                          \<sqsubseteq> Abs_ubundle([ar \<mapsto> tsMap Bool\<cdot> (fst (tsRec\<cdot>(tsMap invBoolPair\<cdot>(ta . dr)))),
-                              abpOut \<mapsto> tsMap Data\<cdot> (snd (tsRec\<cdot>(tsMap invBoolPair\<cdot>(ta . dr))))])"
+      assume a2: "ubclDom\<cdot>(\<Squnion>i. Y i) = {c_dr}"
+      have f3: "\<forall>t ta. (ubclDom\<cdot>t \<noteq> {c_dr} \<or> t \<notsqsubseteq> ta)
+                        \<or> Abs_ubundle([c_ar \<mapsto> tsMap Bool\<cdot> (fst (tsRec\<cdot>(tsMap invBoolPair\<cdot>(t . c_dr)))),
+                            c_abpOut \<mapsto> tsMap Data\<cdot> (snd (tsRec\<cdot> (tsMap invBoolPair\<cdot> (t . c_dr)))::'a tstream)])
+                          \<sqsubseteq> Abs_ubundle([c_ar \<mapsto> tsMap Bool\<cdot> (fst (tsRec\<cdot>(tsMap invBoolPair\<cdot>(ta . c_dr)))),
+                              c_abpOut \<mapsto> tsMap Data\<cdot> (snd (tsRec\<cdot>(tsMap invBoolPair\<cdot>(ta . c_dr))))])"
         using rec_tsb_mono by blast
-      have f4: "\<forall>f n. \<not> chain f \<or> ubDom\<cdot>(f n::'a MABP tstream\<^sup>\<Omega>) = ubDom\<cdot>(Lub f)"
+      have f4: "\<forall>f n. \<not> chain f \<or> ubclDom\<cdot>(f n::'a MABP tstream\<^sup>\<Omega>) = ubclDom\<cdot>(Lub f)"
         using ubdom_chain_eq2 by blast
-      have f5: "\<And> elem_1 .ubDom\<cdot> (Abs_ubundle([ar \<mapsto> tsMap Bool\<cdot> (fst (tsRec\<cdot>(tsMap invBoolPair\<cdot>(Y elem_1 . dr))))
-                          , abpOut \<mapsto> tsMap Data\<cdot> (snd (tsRec\<cdot> (tsMap invBoolPair\<cdot>(Y elem_1 . dr))))]))
-                          = {ar, abpOut}"
+      have f5: "\<And> elem_1 .ubclDom\<cdot> (Abs_ubundle([c_ar \<mapsto> tsMap Bool\<cdot> (fst (tsRec\<cdot>(tsMap invBoolPair\<cdot>(Y elem_1 . c_dr))))
+                          , c_abpOut \<mapsto> tsMap Data\<cdot> (snd (tsRec\<cdot> (tsMap invBoolPair\<cdot>(Y elem_1 . c_dr))))]))
+                          = {c_ar, c_abpOut}"
         by (simp add: recv_tsb_dom)
-      have "\<And> v1_0. ubDom\<cdot> (Y (v1_0 (\<lambda>n. Abs_ubundle([ar \<mapsto> tsMap Bool\<cdot> (fst (tsRec\<cdot>(tsMap invBoolPair\<cdot>(Y n . dr)))),
-                                           abpOut \<mapsto> tsMap Data\<cdot> (snd (tsRec\<cdot> (tsMap invBoolPair\<cdot>(Y n . dr))))])))) = {dr}"
+      have "\<And> v1_0. ubclDom\<cdot> (Y (v1_0 (\<lambda>n. Abs_ubundle([c_ar \<mapsto> tsMap Bool\<cdot> (fst (tsRec\<cdot>(tsMap invBoolPair\<cdot>(Y n . c_dr)))),
+                                           c_abpOut \<mapsto> tsMap Data\<cdot> (snd (tsRec\<cdot> (tsMap invBoolPair\<cdot>(Y n . c_dr))))])))) = {c_dr}"
         using f4 a2 a1 by presburger
-      then have "chain (\<lambda>n. Abs_ubundle([ar \<mapsto> tsMap Bool\<cdot> (fst (tsRec\<cdot>(tsMap invBoolPair\<cdot>(Y n . dr)))),
-                             abpOut \<mapsto> tsMap Data\<cdot> (snd (tsRec\<cdot>(tsMap invBoolPair\<cdot>(Y n . dr))))]))"
+      then have "chain (\<lambda>n. Abs_ubundle([c_ar \<mapsto> tsMap Bool\<cdot> (fst (tsRec\<cdot>(tsMap invBoolPair\<cdot>(Y n . c_dr)))),
+                             c_abpOut \<mapsto> tsMap Data\<cdot> (snd (tsRec\<cdot>(tsMap invBoolPair\<cdot>(Y n . c_dr))))]))"
         using f3 a1 by (simp add: po_class.chain_def)
-      then show "ubDom\<cdot> (\<Squnion>n. Abs_ubundle([ar \<mapsto> tsMap Bool\<cdot> (fst (tsRec\<cdot>(tsMap invBoolPair\<cdot>(Y n . dr)))),
-                               abpOut \<mapsto> tsMap Data\<cdot> (snd (tsRec\<cdot>(tsMap invBoolPair\<cdot>(Y n . dr))))])) = {abpOut, ar}"
+      then show "ubclDom\<cdot> (\<Squnion>n. Abs_ubundle([c_ar \<mapsto> tsMap Bool\<cdot> (fst (tsRec\<cdot>(tsMap invBoolPair\<cdot>(Y n . c_dr)))),
+                               c_abpOut \<mapsto> tsMap Data\<cdot> (snd (tsRec\<cdot>(tsMap invBoolPair\<cdot>(Y n . c_dr))))])) = {c_abpOut, c_ar}"
         using f5 f4 by blast
     qed
 
 
-    have f3: "\<And>(Y::nat \<Rightarrow> 'a MABP tstream\<^sup>\<Omega>) c::channel. chain Y \<Longrightarrow> ubDom\<cdot>(\<Squnion>i::nat. Y i) = {dr}
-              \<Longrightarrow> c = ar \<or> c = abpOut \<Longrightarrow> c = ar \<longrightarrow>
-              (tsMap::(bool \<Rightarrow> 'a MABP) \<Rightarrow> bool tstream \<rightarrow> 'a MABP tstream) Bool\<cdot>(fst (tsRec\<cdot>(tsMap invBoolPair\<cdot>(Lub Y  .  dr))))
-              \<sqsubseteq> (\<Squnion>i::nat. tsMap Bool\<cdot>(fst (tsRec\<cdot>(tsMap invBoolPair\<cdot>(Y i  .  dr)))))"
+    have f3: "\<And>(Y::nat \<Rightarrow> 'a MABP tstream\<^sup>\<Omega>) c::channel. chain Y \<Longrightarrow> ubclDom\<cdot>(\<Squnion>i::nat. Y i) = {c_dr}
+              \<Longrightarrow> c = c_ar \<or> c = c_abpOut \<Longrightarrow> c = c_ar \<longrightarrow>
+              (tsMap::(bool \<Rightarrow> 'a MABP) \<Rightarrow> bool tstream \<rightarrow> 'a MABP tstream) Bool\<cdot>(fst (tsRec\<cdot>(tsMap invBoolPair\<cdot>(Lub Y  .  c_dr))))
+              \<sqsubseteq> (\<Squnion>i::nat. tsMap Bool\<cdot>(fst (tsRec\<cdot>(tsMap invBoolPair\<cdot>(Y i  .  c_dr)))))"
      by (simp add: recvCH1_contlub to_recvch1)
 
-   have f4: "\<And>(Y::nat \<Rightarrow> 'a MABP tstream\<^sup>\<Omega>) c::channel. chain Y \<Longrightarrow> ubDom\<cdot>(\<Squnion>i::nat. Y i) = {dr}
-               \<Longrightarrow> c = ar \<or> c = abpOut \<Longrightarrow> c = ar \<longrightarrow>
-              tsMap Data\<cdot>(snd (tsRec\<cdot>(tsMap invBoolPair\<cdot>(Lub Y  .  dr))))
-               \<sqsubseteq> (\<Squnion>i::nat. tsMap Data\<cdot>(snd (tsRec\<cdot>(tsMap invBoolPair\<cdot>(Y i  .  dr)))))"
+   have f4: "\<And>(Y::nat \<Rightarrow> 'a MABP tstream\<^sup>\<Omega>) c::channel. chain Y \<Longrightarrow> ubclDom\<cdot>(\<Squnion>i::nat. Y i) = {c_dr}
+               \<Longrightarrow> c = c_ar \<or> c = c_abpOut \<Longrightarrow> c = c_ar \<longrightarrow>
+              tsMap Data\<cdot>(snd (tsRec\<cdot>(tsMap invBoolPair\<cdot>(Lub Y  .  c_dr))))
+               \<sqsubseteq> (\<Squnion>i::nat. tsMap Data\<cdot>(snd (tsRec\<cdot>(tsMap invBoolPair\<cdot>(Y i  .  c_dr)))))"
     by (simp add: recvCH2_contlub to_recvch2)
 
   show "\<And>Y::nat \<Rightarrow> 'a MABP tstream\<^sup>\<Omega>.
        chain Y \<Longrightarrow>
-       ubDom\<cdot>(\<Squnion>i::nat. Y i) = {dr} \<Longrightarrow>
-       Abs_ubundle([ar \<mapsto> tsMap Bool\<cdot>(fst (tsRec\<cdot>(tsMap invBoolPair\<cdot>((\<Squnion>i::nat. Y i)  .  dr)))), abpOut \<mapsto>
-        tsMap Data\<cdot>(snd (tsRec\<cdot>(tsMap invBoolPair\<cdot>((\<Squnion>i::nat. Y i)  .  dr))))]) \<sqsubseteq>
+       ubclDom\<cdot>(\<Squnion>i::nat. Y i) = {c_dr} \<Longrightarrow>
+       Abs_ubundle([c_ar \<mapsto> tsMap Bool\<cdot>(fst (tsRec\<cdot>(tsMap invBoolPair\<cdot>((\<Squnion>i::nat. Y i)  .  c_dr)))), c_abpOut \<mapsto>
+        tsMap Data\<cdot>(snd (tsRec\<cdot>(tsMap invBoolPair\<cdot>((\<Squnion>i::nat. Y i)  .  c_dr))))]) \<sqsubseteq>
        (\<Squnion>i::nat.
-           Abs_ubundle([ar \<mapsto> tsMap Bool\<cdot>(fst (tsRec\<cdot>(tsMap invBoolPair\<cdot>(Y i  .  dr)))), abpOut \<mapsto>
-            tsMap Data\<cdot>(snd (tsRec\<cdot>(tsMap invBoolPair\<cdot>(Y i  .  dr))))]))"
+           Abs_ubundle([c_ar \<mapsto> tsMap Bool\<cdot>(fst (tsRec\<cdot>(tsMap invBoolPair\<cdot>(Y i  .  c_dr)))), c_abpOut \<mapsto>
+            tsMap Data\<cdot>(snd (tsRec\<cdot>(tsMap invBoolPair\<cdot>(Y i  .  c_dr))))]))"
       apply (rule ub_below)
        apply (simp_all add: ubdom_below ubdom_ubrep_eq ubgetch_ubrep_eq f1)
       apply (simp add: recvTSPF_tsb_getc ubdom_ubrep_eq ubgetch_ubrep_eq)
@@ -364,53 +331,60 @@ qed
   subsubsection \<open>tspf_well\<close>
 
  (* show that the recvTSPF fulfills the tickcount property *)
-lemma recvTSPF_tick: assumes "ubDom\<cdot>b = {dr}" and "(ubLen b) = n"
-  shows "n \<le> (ubLen (Abs_ubundle([ar \<mapsto> tsMap Bool\<cdot>(fst (tsRec\<cdot>(tsMap invBoolPair\<cdot>(b  .  dr)))),
-                       abpOut \<mapsto> tsMap Data\<cdot>(snd (tsRec\<cdot>(tsMap invBoolPair\<cdot>(b  .  dr))))])))"
+lemma recvTSPF_tick: assumes "ubDom\<cdot>b = {c_dr}" and "(ubLen b) = n"
+  shows "n \<le> (ubLen (Abs_ubundle([c_ar \<mapsto> tsMap Bool\<cdot>(fst (tsRec\<cdot>(tsMap invBoolPair\<cdot>(b  .  c_dr)))),
+                       c_abpOut \<mapsto> tsMap Data\<cdot>(snd (tsRec\<cdot>(tsMap invBoolPair\<cdot>(b  .  c_dr))))])))"
 proof -
-  have "(ubLen b) = #\<surd>(b . dr)"
-    sorry
-(*
-    apply (rule tsbtick_single_ch2)
-     by (simp add: assms(1)) *)
-  hence f1: "n = #\<surd>(b . dr)"
-     using assms(2) by blast
-  hence f2: "n \<le> #\<surd>(tsMap Bool\<cdot>(fst (tsRec\<cdot>(tsMap invBoolPair\<cdot>(b  .  dr)))))"
+  have "(ubLen b) = usclLen\<cdot>(b . c_dr)"
+  proof (simp add: ubLen_def)
+    have "(LEAST l. l \<in> {usclLen\<cdot>(b . c) |c. c \<in> ubDom\<cdot>b}) \<in> {usclLen\<cdot>(b . c) |c. c \<in> ubDom\<cdot>b} \<or> ubDom\<cdot>b = {}"
+      using ublen_least_in_set by blast
+    then have "{c_dr} = {} \<or> (\<exists>c. (LEAST l. \<exists>c. l = usclLen\<cdot>(b . c) \<and> c \<in> ubDom\<cdot>b) = usclLen\<cdot>(b . c) \<and> c \<in> ubDom\<cdot>b)"
+      by (simp add: assms(1))
+    then show "(ubDom\<cdot>b \<noteq> {} \<longrightarrow> (LEAST l. \<exists>c. l = usclLen\<cdot>(b . c) \<and> c \<in> ubDom\<cdot>b) = usclLen\<cdot>(b . c_dr)) \<and> (ubDom\<cdot>b = {} \<longrightarrow> \<infinity> = usclLen\<cdot>(b . c_dr))"
+      by (simp add: assms(1))
+  qed
+  hence f1: "n = #\<surd>(b . c_dr)"
+    by (metis assms(2) usclLen_tstream_def)
+  hence f2: "n \<le> #\<surd>(tsMap Bool\<cdot>(fst (tsRec\<cdot>(tsMap invBoolPair\<cdot>(b  .  c_dr)))))"
     by (simp add: tsrec_insert)
-  with f1 have f3: "n \<le> #\<surd>(tsMap Data\<cdot>(snd (tsRec\<cdot>(tsMap invBoolPair\<cdot>(b  .  dr)))))"
+  with f1 have f3: "n \<le> #\<surd>(tsMap Data\<cdot>(snd (tsRec\<cdot>(tsMap invBoolPair\<cdot>(b  .  c_dr)))))"
     by (simp add: tsrec_insert)
+  have f4: "ubDom\<cdot>(Abs_ubundle [c_ar \<mapsto> tsMap Bool\<cdot>(fst (tsRec\<cdot>(tsMap invBoolPair\<cdot>(b  .  c_dr)))), c_abpOut \<mapsto> tsMap Data\<cdot>(snd (tsRec\<cdot>(tsMap invBoolPair\<cdot>(b  .  c_dr))))])
+    = {c_ar, c_abpOut}"
+    by (metis recv_tsb_dom ubclDom_ubundle_def)
   show ?thesis 
-    sorry
-(*
-    apply (rule tsbtick_geI)
-      apply (simp_all add: recv_tsb_dom)
-      apply (simp add: tsbgetch_rep_eq)
-      using f2 f3 by auto *)
+    apply (rule ubLen_geI)
+      apply (simp_all add: f4)
+    apply (simp add: ubgetch_ubrep_eq)
+    by (metis f2 f3 usclLen_tstream_def)
 qed
 
 
   (* recvTSPF is an actual TSPF *)
 lemma recvTSPF_well [simp]:
-  shows "ufWell (\<Lambda> x. (ubDom\<cdot>x = {dr}) \<leadsto>
-                      Abs_ubundle([ar \<mapsto> (tsMap::(bool \<Rightarrow> 'a MABP) \<Rightarrow> bool tstream \<rightarrow> 'a MABP tstream)
+  shows "ufWell (\<Lambda> x. (ubclDom\<cdot>x = {c_dr}) \<leadsto>
+                      Abs_ubundle([c_ar \<mapsto> (tsMap::(bool \<Rightarrow> 'a MABP) \<Rightarrow> bool tstream \<rightarrow> 'a MABP tstream)
                             Bool\<cdot>(fst ((tsRec::('a * bool) tstream \<rightarrow> (bool tstream \<times> 'a tstream))\<cdot>
-                            ((tsMap invBoolPair)\<cdot>(x . dr)))),
-                       abpOut \<mapsto> (tsMap::('a \<Rightarrow> 'a MABP) \<Rightarrow> 'a tstream \<rightarrow> 'a MABP tstream)
-                            Data\<cdot>(snd (tsRec\<cdot>((tsMap invBoolPair)\<cdot>(x . dr))))]))"
-  sorry 
- (*
-    apply (rule ufun_wellI)
-    apply (simp_all add: domIff2 recv_tsb_dom)
-    by (simp add: recvTSPF_tick) *)
+                            ((tsMap invBoolPair)\<cdot>(x . c_dr)))),
+                       c_abpOut \<mapsto> (tsMap::('a \<Rightarrow> 'a MABP) \<Rightarrow> 'a tstream \<rightarrow> 'a MABP tstream)
+                            Data\<cdot>(snd (tsRec\<cdot>((tsMap invBoolPair)\<cdot>(x . c_dr))))]))"
+  apply (rule ufun_wellI)
+  by (simp_all add: domIff2 recv_tsb_dom)
 
 lemma recv_revsubst: "Abs_cufun (recvAbb) = recvTSPF"
   by (simp add: recvTSPF_def)
     
-lemma recv_tspfdom: "ufDom\<cdot>(recvTSPF) = {dr}"
-  by (rule recvTSPF_well)
-   
-lemma recv_tspfran: "ufRan\<cdot>(recvTSPF) = {ar, abpOut}"
-  by (rule recvTSPF_well)
+lemma recv_tspfdom: "ufDom\<cdot>(recvTSPF) = {c_dr}"
+  apply (simp add: ufDom_def recvTSPF_def)
+  apply (simp add: domIff)
+  by (simp add: ubclDom_h)
+
+lemma recv_tspfran: "ufRan\<cdot>(recvTSPF) = {c_ar, c_abpOut}"
+  apply (simp add: ufran_least)
+    apply (subst recv_tspfdom)
+    apply (simp only: recvTSPF_def)
+  by (simp add:  recv_tsb_dom ubcldom_least_cs) 
 
 
   subsection \<open>medium_rs\<close>
@@ -418,18 +392,18 @@ lemma recv_tspfran: "ufRan\<cdot>(recvTSPF) = {ar, abpOut}"
 (*
 
 definition tsMedRSTSPF :: "bool stream \<Rightarrow> 'a MABP TSPF" where
-"tsMedRSTSPF bst\<equiv> Abs_CTSPF (\<lambda> x. (tsbDom\<cdot>x = {ar})
-                           \<leadsto> [as \<mapsto> (tsMap::(bool \<Rightarrow> 'a MABP) \<Rightarrow> bool tstream \<rightarrow> 'a MABP tstream) Bool\<cdot>(tsMed\<cdot>(tsMap invBool\<cdot>(x . ar))\<cdot>bst)]\<Omega>)"
+"tsMedRSTSPF bst\<equiv> Abs_CTSPF (\<lambda> x. (tsbDom\<cdot>x = {c_ar})
+                           \<leadsto> [c_as \<mapsto> (tsMap::(bool \<Rightarrow> 'a MABP) \<Rightarrow> bool tstream \<rightarrow> 'a MABP tstream) Bool\<cdot>(tsMed\<cdot>(tsMap invBool\<cdot>(x . c_ar))\<cdot>bst)]\<Omega>)"
 
 abbreviation tsMedRSAbb  :: "bool stream \<Rightarrow> 'a MABP TSB \<Rightarrow> 'a MABP TSB option" where
-"tsMedRSAbb bst x \<equiv> ((tsbDom\<cdot>x = {ar})
-                           \<leadsto> [as \<mapsto> (tsMap::(bool \<Rightarrow> 'a MABP) \<Rightarrow> bool tstream \<rightarrow> 'a MABP tstream) Bool\<cdot>(tsMed\<cdot>(tsMap invBool\<cdot>(x . ar))\<cdot>bst)]\<Omega>)"
+"tsMedRSAbb bst x \<equiv> ((tsbDom\<cdot>x = {c_ar})
+                           \<leadsto> [c_as \<mapsto> (tsMap::(bool \<Rightarrow> 'a MABP) \<Rightarrow> bool tstream \<rightarrow> 'a MABP tstream) Bool\<cdot>(tsMed\<cdot>(tsMap invBool\<cdot>(x . c_ar))\<cdot>bst)]\<Omega>)"
 
 *)
 subsubsection \<open>defs\<close>
 
-definition medRSH :: "bool stream \<Rightarrow> 'a MABP TSB \<Rightarrow> 'a MABP tstream"  where
-"medRSH bst \<equiv> (\<lambda> x. (tsMap::(bool \<Rightarrow> 'a MABP) \<Rightarrow> bool tstream \<rightarrow> 'a MABP tstream) Bool\<cdot>(tsMed\<cdot>(tsMap invBool\<cdot>(x  .  ar))\<cdot>bst))"
+definition medRSH :: "bool stream \<Rightarrow> 'a MABP tstream\<^sup>\<Omega> \<Rightarrow> 'a MABP tstream"  where
+"medRSH bst \<equiv> (\<lambda> x. (tsMap::(bool \<Rightarrow> 'a MABP) \<Rightarrow> bool tstream \<rightarrow> 'a MABP tstream) Bool\<cdot>(tsMed\<cdot>(tsMap invBool\<cdot>(x  .  c_ar))\<cdot>bst))"
 
 lemma medrsh_cont [simp]: "cont (medRSH bst)"
   by (simp add: medRSH_def)
@@ -439,8 +413,8 @@ lemma medrsh_contlub: assumes "chain Y"
   apply (rule cont2contlubE)
   by (simp_all add: assms)
 
-lemma to_medrsh: "tsMap Bool\<cdot>(tsMed\<cdot>(tsMap invBool\<cdot>(x  .  ar))\<cdot>bst)
-                  = ((medRSH :: bool stream \<Rightarrow> 'a MABP TSB \<Rightarrow> 'a MABP tstream) bst) x"
+lemma to_medrsh: "tsMap Bool\<cdot>(tsMed\<cdot>(tsMap invBool\<cdot>(x  .  c_ar))\<cdot>bst)
+                  = ((medRSH :: bool stream \<Rightarrow> 'a MABP tstream\<^sup>\<Omega> \<Rightarrow> 'a MABP tstream) bst) x"
   by (simp add: medRSH_def)
 
 subsubsection \<open>pre\<close>
@@ -452,146 +426,156 @@ lemma tsmed_input_mono [simp]: "monofun (\<lambda> x. tsMed\<cdot>x\<cdot>bst)"
   using cont2mono tsmed_input_cont by blast
 
 
-lemma medrs_tsb_well [simp]: "tsb_well  [as \<mapsto> tsMap Bool\<cdot>(tsMed\<cdot>(tsMap invBool\<cdot>(x . ar))\<cdot>bst)]"
-  apply (rule tsb_wellI)
+lemma medrs_tsb_well [simp]: "ubWell  [c_as \<mapsto> tsMap Bool\<cdot>(tsMed\<cdot>(tsMap invBool\<cdot>(x . c_ar))\<cdot>bst)]"
+  apply (rule ubwellI)
+  apply (simp add: usclOkay_tstream_def)
   by (simp add: tsmap_tsdom_range)
 
-lemma medrs_tsb_dom: "tsbDom\<cdot>([as \<mapsto> tsMap Bool\<cdot>(tsMed\<cdot>(tsMap invBool\<cdot>(x . ar))\<cdot>bst)]\<Omega>) = {as}"
-  by (simp add: tsbdom_rep_eq)
+lemma medrs_tsb_dom: "ubclDom\<cdot>(Abs_ubundle([c_as \<mapsto> tsMap Bool\<cdot>(tsMed\<cdot>(tsMap invBool\<cdot>(x . c_ar))\<cdot>bst)])) = {c_as}"
+  apply (simp add: ubclDom_ubundle_def)
+  by (simp add: ubdom_ubrep_eq)
 
 
 subsubsection \<open>cont\<close>
 
   (* prerequirement for the mono proofs of the tspf *)
-lemma medrs_tsb_mono: "\<And>(x::'a MABP TSB) y::'a MABP TSB.
-       tsbDom\<cdot>x = {ar} \<Longrightarrow> x \<sqsubseteq> y \<Longrightarrow> [as \<mapsto> (tsMap::(bool \<Rightarrow> 'a MABP) \<Rightarrow> bool tstream \<rightarrow> 'a MABP tstream) Bool\<cdot>(tsMed\<cdot>(tsMap invBool\<cdot>(x  .  ar))\<cdot>bst)]\<Omega> \<sqsubseteq> [as \<mapsto> tsMap Bool\<cdot>(tsMed\<cdot>(tsMap invBool\<cdot>(y  .  ar))\<cdot>bst)]\<Omega>"
-  apply (simp_all add: tsbdom_below tsbdom_rep_eq tsbgetch_rep_eq)
-  apply (rule tsb_below)
-    apply (simp_all add: tsbdom_below tsbdom_rep_eq  tsbgetch_rep_eq)
-    apply (simp add: to_medrsh)
-    using cont2mono medrsh_cont monofun_def by blast
+lemma medrs_tsb_mono: "\<And>(x::'a MABP tstream\<^sup>\<Omega>) y::'a MABP tstream\<^sup>\<Omega>.
+       ubclDom\<cdot>x = {c_ar} \<Longrightarrow> x \<sqsubseteq> y \<Longrightarrow> Abs_ubundle([c_as \<mapsto> (tsMap::(bool \<Rightarrow> 'a MABP) \<Rightarrow> bool tstream \<rightarrow> 'a MABP tstream) Bool\<cdot>(tsMed\<cdot>(tsMap invBool\<cdot>(x  .  c_ar))\<cdot>bst)]) \<sqsubseteq> Abs_ubundle([c_as \<mapsto> tsMap Bool\<cdot>(tsMed\<cdot>(tsMap invBool\<cdot>(y  .  c_ar))\<cdot>bst)])"
+  apply (simp_all add: ubclDom_ubundle_def)
+  apply (rule ub_below)
+  apply (simp_all add: ubdom_below ubdom_ubrep_eq ubgetch_ubrep_eq)
+  apply (simp add: to_medrsh)
+  using cont2mono medrsh_cont monofun_def by blast
 
 
-lemma medrs_mono [simp]: "monofun (\<lambda> x::'a MABP TSB. (tsbDom\<cdot>x = {ar})
-                           \<leadsto> [as \<mapsto> (tsMap::(bool \<Rightarrow> 'a MABP) \<Rightarrow> bool tstream \<rightarrow> 'a MABP tstream)
-                                Bool\<cdot>(tsMed\<cdot>(tsMap invBool\<cdot>(x . ar))\<cdot>bst)]\<Omega>)"
-  apply (rule tspf_monoI)
+lemma medrs_mono [simp]: "monofun (\<lambda> x::'a MABP tstream\<^sup>\<Omega>. (ubclDom\<cdot>x = {c_ar})
+                           \<leadsto> Abs_ubundle([c_as \<mapsto> (tsMap::(bool \<Rightarrow> 'a MABP) \<Rightarrow> bool tstream \<rightarrow> 'a MABP tstream)
+                                Bool\<cdot>(tsMed\<cdot>(tsMap invBool\<cdot>(x . c_ar))\<cdot>bst)]))"
+  apply (rule ufun_monoI2)
   by (simp add: medrs_tsb_mono)
 
-lemma medrs_tsb_getc: assumes "chain (Y::nat \<Rightarrow> 'a MABP TSB)" and "tsbDom\<cdot>(\<Squnion>i::nat. Y i) = {ar}"
-                      and "c = as"
-  shows "(\<Squnion>i::nat. [as \<mapsto> (tsMap::(bool \<Rightarrow> 'a MABP) \<Rightarrow> bool tstream \<rightarrow> 'a MABP tstream) Bool\<cdot>(tsMed\<cdot>(tsMap invBool\<cdot>(Y i  .  ar))\<cdot>bst)]\<Omega>)  .  as
-          =  (\<Squnion>i::nat. ([as \<mapsto> (tsMap::(bool \<Rightarrow> 'a MABP) \<Rightarrow> bool tstream \<rightarrow> 'a MABP tstream) Bool\<cdot>(tsMed\<cdot>(tsMap invBool\<cdot>(Y i  .  ar))\<cdot>bst)]\<Omega>) . as)"
+lemma medrs_tsb_getc: assumes "chain (Y::nat \<Rightarrow> 'a MABP tstream\<^sup>\<Omega>)" and "ubclDom\<cdot>(\<Squnion>i::nat. Y i) = {c_ar}"
+                      and "c = c_as"
+  shows "(\<Squnion>i::nat. Abs_ubundle([c_as \<mapsto> (tsMap::(bool \<Rightarrow> 'a MABP) \<Rightarrow> bool tstream \<rightarrow> 'a MABP tstream) Bool\<cdot>(tsMed\<cdot>(tsMap invBool\<cdot>(Y i  .  c_ar))\<cdot>bst)]))  .  c_as
+          =  (\<Squnion>i::nat. (Abs_ubundle([c_as \<mapsto> (tsMap::(bool \<Rightarrow> 'a MABP) \<Rightarrow> bool tstream \<rightarrow> 'a MABP tstream) Bool\<cdot>(tsMed\<cdot>(tsMap invBool\<cdot>(Y i  .  c_ar))\<cdot>bst)])) . c_as)"
 proof (rule lubgetCh)
-  have f2: "\<And> i. tsbDom\<cdot>(Y i) =  tsbDom\<cdot>(\<Squnion>i. Y i)"
-    by (simp add: assms(1))
-  show tb_chain: "chain (\<lambda>i::nat. [as \<mapsto> (tsMap::(bool \<Rightarrow> 'a MABP) \<Rightarrow> bool tstream \<rightarrow> 'a MABP tstream) Bool\<cdot>(tsMed\<cdot>(tsMap invBool\<cdot>(Y i  .  ar))\<cdot>bst)]\<Omega>)"
-    by (simp add: assms(1) assms(2) po_class.chainE po_class.chainI medrs_tsb_mono)
-  show "as \<in> tsbDom\<cdot>(\<Squnion>i::nat. [as \<mapsto> (tsMap::(bool \<Rightarrow> 'a MABP) \<Rightarrow> bool tstream \<rightarrow> 'a MABP tstream) Bool\<cdot>(tsMed\<cdot>(tsMap invBool\<cdot>(Y i  .  ar))\<cdot>bst)]\<Omega>)"
-    using assms(3) medrs_tsb_dom tb_chain tsbChain_dom_eq2 by blast
+  have f2: "\<And> i. ubclDom\<cdot>(Y i) =  ubclDom\<cdot>(\<Squnion>i. Y i)"
+    by (simp add: assms(1) ubclDom_ubundle_def)
+  show tb_chain: "chain (\<lambda>i::nat. Abs_ubundle([c_as \<mapsto> (tsMap::(bool \<Rightarrow> 'a MABP) \<Rightarrow> bool tstream \<rightarrow> 'a MABP tstream) Bool\<cdot>(tsMed\<cdot>(tsMap invBool\<cdot>(Y i  .  c_ar))\<cdot>bst)]))"
+    by (simp add: assms(1) assms(2) f2 medrs_tsb_mono po_class.chainE po_class.chainI)
+  show "c_as \<in> ubclDom\<cdot>(\<Squnion>i::nat. Abs_ubundle([c_as \<mapsto> (tsMap::(bool \<Rightarrow> 'a MABP) \<Rightarrow> bool tstream \<rightarrow> 'a MABP tstream) Bool\<cdot>(tsMed\<cdot>(tsMap invBool\<cdot>(Y i  .  c_ar))\<cdot>bst)]))"
+    by (metis (mono_tags, lifting) insert_iff medrs_tsb_dom tb_chain ubclDom_ubundle_def ubdom_chain_eq2)
 qed
 
 
 
-lemma medrs_cont [simp]: "cont (\<lambda> x::'a MABP TSB. (tsbDom\<cdot>x = {ar})
-                           \<leadsto> [as \<mapsto> (tsMap::(bool \<Rightarrow> 'a MABP) \<Rightarrow> bool tstream \<rightarrow> 'a MABP tstream)
-                                Bool\<cdot>(tsMed\<cdot>(tsMap invBool\<cdot>(x . ar))\<cdot>bst)]\<Omega>)"
-proof (rule tspf_contI)
-  show medrs_mo : "\<And>(x::'a MABP TSB) y::'a MABP TSB. tsbDom\<cdot>x = {ar} \<Longrightarrow> x \<sqsubseteq> y \<Longrightarrow>
-          [as \<mapsto> (tsMap::(bool \<Rightarrow> 'a MABP) \<Rightarrow> bool tstream \<rightarrow> 'a MABP tstream) Bool\<cdot>
-                  (tsMed\<cdot>(tsMap invBool\<cdot>(x  .  ar))\<cdot>bst)]\<Omega>
-          \<sqsubseteq> [as \<mapsto> tsMap Bool\<cdot>(tsMed\<cdot>(tsMap invBool\<cdot>(y  .  ar))\<cdot>bst)]\<Omega>"
-    by (simp add: medrs_tsb_mono)
+lemma medrs_cont [simp]: "cont (\<lambda> x::'a MABP tstream\<^sup>\<Omega>. (ubclDom\<cdot>x = {c_ar})
+                           \<leadsto> Abs_ubundle([c_as \<mapsto> (tsMap::(bool \<Rightarrow> 'a MABP) \<Rightarrow> bool tstream \<rightarrow> 'a MABP tstream)
+                                Bool\<cdot>(tsMed\<cdot>(tsMap invBool\<cdot>(x . c_ar))\<cdot>bst)]))"
+proof (rule ufun_contI)
+  show medrs_mo : "\<And>(x::'a MABP tstream\<^sup>\<Omega>) y::'a MABP tstream\<^sup>\<Omega>.
+       ubclDom\<cdot>x = {c_ar} \<Longrightarrow> x \<sqsubseteq> y \<Longrightarrow> Abs_ubundle [c_as \<mapsto> tsMap Bool\<cdot>(tsMed\<cdot>(tsMap invBool\<cdot>(x  .  c_ar))\<cdot>bst)] 
+          \<sqsubseteq> Abs_ubundle [c_as \<mapsto> tsMap Bool\<cdot>(tsMed\<cdot>(tsMap invBool\<cdot>(y  .  c_ar))\<cdot>bst)]"
+    by (simp add: medrs_tsb_well monofun_cfun_arg monofun_cfun_fun option.distinct(1) option.sel ub_below ubdom_ubrep_eq ubgetch_ubrep_eq)
 
-  have f1: " \<And>Y::nat \<Rightarrow> 'a MABP TSB. chain Y \<Longrightarrow> tsbDom\<cdot>(\<Squnion>i::nat. Y i) = {ar} \<Longrightarrow>
-       tsbDom\<cdot>(\<Squnion>i::nat. [as \<mapsto> (tsMap::(bool \<Rightarrow> 'a MABP) \<Rightarrow> bool tstream \<rightarrow> 'a MABP tstream) Bool\<cdot>(tsMed\<cdot>(tsMap invBool\<cdot>(Y i  .  ar))\<cdot>bst)]\<Omega>) = {as}"
-    by (metis (mono_tags, lifting) medrs_mo medrs_tsb_dom po_class.chainE po_class.chainI tsbChain_dom_eq2)
-
-
-  show "\<And>Y::nat \<Rightarrow> 'a MABP TSB. chain Y \<Longrightarrow> tsbDom\<cdot>(\<Squnion>i::nat. Y i) = {ar} \<Longrightarrow>
-       [as \<mapsto> (tsMap::(bool \<Rightarrow> 'a MABP) \<Rightarrow> bool tstream \<rightarrow> 'a MABP tstream) Bool\<cdot>(tsMed\<cdot>(tsMap invBool\<cdot>((\<Squnion>i::nat. Y i)  .  ar))\<cdot>bst)]\<Omega> \<sqsubseteq> (\<Squnion>i::nat. [as \<mapsto> tsMap Bool\<cdot>(tsMed\<cdot>(tsMap invBool\<cdot>(Y i  .  ar))\<cdot>bst)]\<Omega>)"
-    apply (rule tsb_below)
-      apply (simp_all add: tsbdom_below tsbdom_rep_eq tsbgetch_rep_eq f1)
-      apply (simp add: medrs_tsb_getc tsbdom_rep_eq tsbgetch_rep_eq)
-       by (simp add: medrsh_contlub to_medrsh)
+  have f1: " \<And>Y::nat \<Rightarrow> 'a MABP tstream\<^sup>\<Omega>. chain Y \<Longrightarrow> ubclDom\<cdot>(\<Squnion>i::nat. Y i) = {c_ar} \<Longrightarrow>
+       ubclDom\<cdot>(\<Squnion>i::nat. Abs_ubundle([c_as \<mapsto> (tsMap::(bool \<Rightarrow> 'a MABP) \<Rightarrow> bool tstream \<rightarrow> 'a MABP tstream) Bool\<cdot>(tsMed\<cdot>(tsMap invBool\<cdot>(Y i  .  c_ar))\<cdot>bst)])) = {c_as}"
+    by (metis (mono_tags, lifting) medrs_tsb_dom medrs_tsb_mono po_class.chain_def ubcldom_lub_eq2I)
+  show "\<And>Y::nat \<Rightarrow> 'a MABP tstream\<^sup>\<Omega>. chain Y \<Longrightarrow> ubclDom\<cdot>(\<Squnion>i::nat. Y i) = {c_ar} \<Longrightarrow>
+       Abs_ubundle([c_as \<mapsto> (tsMap::(bool \<Rightarrow> 'a MABP) \<Rightarrow> bool tstream \<rightarrow> 'a MABP tstream) Bool\<cdot>(tsMed\<cdot>(tsMap invBool\<cdot>((\<Squnion>i::nat. Y i)  .  c_ar))\<cdot>bst)]) \<sqsubseteq> (\<Squnion>i::nat. Abs_ubundle([c_as \<mapsto> tsMap Bool\<cdot>(tsMed\<cdot>(tsMap invBool\<cdot>(Y i  .  c_ar))\<cdot>bst)]))"
+  proof -
+    fix Y::"nat \<Rightarrow> 'a MABP tstream\<^sup>\<Omega>"
+    assume chain_Y: "chain Y" and chain_Y_dom: "ubclDom\<cdot>(\<Squnion>i::nat. Y i) = {c_ar}"
+    have f10: "(\<Squnion>i::nat. Abs_ubundle [c_as \<mapsto> tsMap Bool\<cdot>(tsMed\<cdot>(tsMap invBool\<cdot>(Y i  .  c_ar))\<cdot>bst)])  .  c_as =
+                    (\<Squnion>i::nat. Abs_ubundle [c_as \<mapsto> tsMap Bool\<cdot>(tsMed\<cdot>(tsMap invBool\<cdot>(Y i  .  c_ar))\<cdot>bst)]  .  c_as)"
+      apply (rule cont2contlubE, simp)
+      apply (rule chainI)
+      by (simp add: chain_Y monofun_cfun_arg monofun_cfun_fun po_class.chainE ub_below ubdom_ubrep_eq ubgetch_ubrep_eq)
+    show "Abs_ubundle([c_as \<mapsto> (tsMap::(bool \<Rightarrow> 'a MABP) \<Rightarrow> bool tstream \<rightarrow> 'a MABP tstream) Bool\<cdot>(tsMed\<cdot>(tsMap invBool\<cdot>((\<Squnion>i::nat. Y i)  .  c_ar))\<cdot>bst)]) \<sqsubseteq> (\<Squnion>i::nat. Abs_ubundle([c_as \<mapsto> tsMap Bool\<cdot>(tsMed\<cdot>(tsMap invBool\<cdot>(Y i  .  c_ar))\<cdot>bst)]))"
+      apply (rule ub_below)
+       apply (simp_all add: ubdom_below ubdom_ubrep_eq ubgetch_ubrep_eq f1) 
+       apply (metis (mono_tags, lifting) chain_Y chain_Y_dom f1 ubclDom_ubundle_def)
+      apply (subst f10)
+      by (metis (mono_tags, lifting) chain_Y fun_upd_same lub_eq medrs_tsb_well medrsh_contlub not_below2not_eq option.sel to_medrsh ubgetch_ubrep_eq)
+  qed
 qed
 
 
   subsubsection \<open>tspf_well\<close>
   
  (* show that the mediumRSTSPF template  fulfills the tickcount property *)
-lemma medrs_tick: assumes "tsbDom\<cdot>b = {ar}" and "(#\<surd>tsb b) = n" and "#bst=\<infinity>"
-  shows "n \<le> (#\<surd>tsb [as \<mapsto> (tsMap::(bool \<Rightarrow> 'a MABP) \<Rightarrow> bool tstream \<rightarrow> 'a MABP tstream) Bool\<cdot>(tsMed\<cdot>(tsMap invBool\<cdot>(b  .  ar))\<cdot>bst)]\<Omega>)"
+lemma medrs_tick: assumes "ubclDom\<cdot>b = {c_ar}" and "(ubLen b) = n" and "#bst=\<infinity>"
+  shows "n \<le> (ubclLen (Abs_ubundle([c_as \<mapsto> (tsMap::(bool \<Rightarrow> 'a MABP) \<Rightarrow> bool tstream \<rightarrow> 'a MABP tstream) Bool\<cdot>(tsMed\<cdot>(tsMap invBool\<cdot>(b  .  c_ar))\<cdot>bst)])))"
 proof -
-  have "(#\<surd>tsb b) = #\<surd>(b . ar)"
-    apply (rule tsbtick_single_ch2)
-    by (simp add: assms(1))
-  hence f1: "n = #\<surd>(b . ar)"
+  have "(ubLen b) = usclLen\<cdot>(b . c_ar)"
+    apply (rule uslen_ubLen_ch3)
+    by (metis assms(1) ubclDom_ubundle_def)
+  hence f1: "n = usclLen\<cdot>(b . c_ar)"
     using assms(2) by blast
-  hence f2: "n \<le> #\<surd>((tsMap::(bool \<Rightarrow> 'a MABP) \<Rightarrow> bool tstream \<rightarrow> 'a MABP tstream) Bool\<cdot>(tsMed\<cdot>(tsMap invBool\<cdot>(b  .  ar))\<cdot>bst))"
-    by (simp add: assms(3))
+  hence f2: "n \<le> usclLen\<cdot>((tsMap::(bool \<Rightarrow> 'a MABP) \<Rightarrow> bool tstream \<rightarrow> 'a MABP tstream) Bool\<cdot>(tsMed\<cdot>(tsMap invBool\<cdot>(b  .  c_ar))\<cdot>bst))"
+    by (simp add: assms(3) usclLen_tstream_def)
   show ?thesis
-    apply (rule tsbtick_geI)
-    apply (simp add: medrs_tsb_dom tsbgetch_rep_eq)
-    using f2 by force
+    apply (simp add: ubclLen_ubundle_def)
+    apply (rule ubLen_geI)
+    apply (simp add: medrs_tsb_dom ubgetch_ubrep_eq)
+    by (simp add: f2 ubdom_ubrep_eq)
 qed
   
       
     
   (* a medium is a tspf if the oracle bool stream bst is infinitly long*)
 lemma medrs_well [simp]: assumes "#bst=\<infinity>"
-  shows "tspf_well (\<Lambda> x. (tsbDom\<cdot>x = {ar})
-                           \<leadsto> [as \<mapsto> (tsMap::(bool \<Rightarrow> 'a MABP) \<Rightarrow> bool tstream \<rightarrow> 'a MABP tstream)
-                                Bool\<cdot>(tsMed\<cdot>(tsMap invBool\<cdot>(x . ar))\<cdot>bst)]\<Omega>)"
-  apply (rule tspf_wellI)
-    apply (simp_all add: domIff2 medrs_tsb_dom)
-    apply (subst tsbtick_single_ch1, simp)
-    by (simp add: assms tsbtick_single_ch2)
+  shows "ufWell (\<Lambda> (x::'a MABP tstream\<^sup>\<Omega>). (ubclDom\<cdot>x = {c_ar})
+                           \<leadsto> Abs_ubundle([c_as \<mapsto> (tsMap::(bool \<Rightarrow> 'a MABP) \<Rightarrow> bool tstream \<rightarrow> 'a MABP tstream)
+                                Bool\<cdot>(tsMed\<cdot>(tsMap invBool\<cdot>(x . c_ar))\<cdot>bst)]))"
+  apply (rule ufun_wellI)
+    apply (simp_all add: domIff2)
+  by (simp add:  ubclDom_ubundle_def ubDom_def)
 
       
-lemma medrs_revsubst: "Abs_CTSPF (tsMedRSAbb bst) = (medRS_TSPF bst)"
+lemma medrs_revsubst: "Abs_cufun (tsMedRSAbb bst) = (medRS_TSPF bst)"
   by (simp add: medRS_TSPF_def)
     
 lemma medrs_tspfdom: assumes "#bst =\<infinity>"
-  shows "tspfDom\<cdot>(medRS_TSPF bst) = {ar}"
+  shows "ufDom\<cdot>(medRS_TSPF bst) = {c_ar}"
     apply (simp add: medRS_TSPF_def)
-    apply (simp add: tspf_dom_insert assms)
+    apply (simp add: ufdom_insert assms)
     apply (simp add: domIff2)
-    by (meson tsbleast_tsdom someI)
+  by (simp add: ubclDom_h)
    
 lemma medrs_tspfran: assumes "#bst =\<infinity>"
-  shows "tspfRan\<cdot>(medRS_TSPF bst) = {as}"   
+  shows "ufRan\<cdot>(medRS_TSPF bst) = {c_as}"   
     apply (simp add: medRS_TSPF_def)
-    apply (simp add: tspfran_least medrs_tspfdom assms)
+    apply (simp add: ufran_least medrs_tspfdom assms)
     apply (simp add: medrs_revsubst medrs_tspfdom assms)
-    by (metis singletonI tsb_newMap_id tsbleast_getch tsbleast_tsdom)
+  by (simp add: medrs_tsb_dom ubcldom_least_cs)
 
 
   (* now special lemmata for TSPS instantiation *)
 
 lemma medrs_well2 [simp]: assumes "#({True} \<ominus> bst) = \<infinity>"
-  shows "tspf_well (\<Lambda> x. (tsbDom\<cdot>x = {ar})
-                           \<leadsto> [as \<mapsto> (tsMap::(bool \<Rightarrow> 'a MABP) \<Rightarrow> bool tstream \<rightarrow> 'a MABP tstream)
-                                Bool\<cdot>(tsMed\<cdot>(tsMap invBool\<cdot>(x . ar))\<cdot>bst)]\<Omega>)"
+  shows "ufWell (\<Lambda> (x::'a MABP tstream\<^sup>\<Omega>). (ubclDom\<cdot>x = {c_ar})
+                           \<leadsto> Abs_ubundle([c_as \<mapsto> (tsMap::(bool \<Rightarrow> 'a MABP) \<Rightarrow> bool tstream \<rightarrow> 'a MABP tstream)
+                                Bool\<cdot>(tsMed\<cdot>(tsMap invBool\<cdot>(x . c_ar))\<cdot>bst)]))"
 proof -
    have "#bst = \<infinity>"
      by (simp add: med_ora_length assms(1))
-   thus ?thesis
+   thus ?thesis  
      by (simp add: medrs_tspfdom)
 qed
   
 
 lemma medrs_tspfdom2: assumes "#({True} \<ominus> bst) = \<infinity>"
-  shows "tspfDom\<cdot>(medRS_TSPF bst) = {ar}"
+  shows "ufclDom\<cdot>(medRS_TSPF bst) = {c_ar}"
 proof -
   have "#bst = \<infinity>"
     by (simp add: med_ora_length assms(1))
   thus ?thesis
-    by (simp add: medrs_tspfdom)
+    by (simp add: medrs_tspfdom ufclDom_ufun_def)
 qed
   
 lemma medrs_tspfran2: assumes "#({True} \<ominus> bst) = \<infinity>"
-  shows "tspfRan\<cdot>(medRS_TSPF bst) = {as}"
+  shows "ufRan\<cdot>(medRS_TSPF bst) = {c_as}"
 proof -
   have "#bst = \<infinity>"
     by (simp add: med_ora_length assms(1))
@@ -600,18 +584,18 @@ proof -
 qed
 
   (* necessary for TSPS instantiation *)
-lemma medrs_tsps_dom1 [simp]: "f = medRS_TSPF ora \<and> #({True} \<ominus> ora) = \<infinity> \<Longrightarrow> tspfDom\<cdot>f = {ar}"
-  by (simp add: medrs_tspfdom2)
+lemma medrs_tsps_dom1 [simp]: "f = medRS_TSPF ora \<and> #({True} \<ominus> ora) = \<infinity> \<Longrightarrow> ufDom\<cdot>f = {c_ar}"
+  by (metis medrs_tspfdom2 ufclDom_ufun_def)
 
 lemma medrs_tsps_dom2 [simp]: "\<exists>ora::bool stream. f = medRS_TSPF ora \<and> #({True} \<ominus> ora) = \<infinity> 
-                               \<Longrightarrow> tspfDom\<cdot>f = {ar}"
+                               \<Longrightarrow> ufDom\<cdot>f = {c_ar}"
   using medrs_tsps_dom1  by auto
  
-lemma medrs_tsps_ran1 [simp]: "f = medRS_TSPF ora \<and> #({True} \<ominus> ora) = \<infinity> \<Longrightarrow> tspfRan\<cdot>f = {as}"
+lemma medrs_tsps_ran1 [simp]: "f = medRS_TSPF ora \<and> #({True} \<ominus> ora) = \<infinity> \<Longrightarrow> ufRan\<cdot>f = {c_as}"
   by (simp add: medrs_tspfran2)
 
 lemma medrs_tsps_ran2 [simp]: "\<exists>ora::bool stream. f = medRS_TSPF ora \<and> #({True} \<ominus> ora) = \<infinity> 
-                               \<Longrightarrow> tspfRan\<cdot>f = {as}"
+                               \<Longrightarrow> ufRan\<cdot>f = {c_as}"
   using medrs_tsps_ran1 by auto
 
 
@@ -622,7 +606,7 @@ subsubsection \<open>defs\<close>
 
 definition medSRH :: "bool stream \<Rightarrow> 'a MABP TSB \<Rightarrow> 'a MABP tstream"  where
 "medSRH bst \<equiv> (\<lambda> x. (tsMap:: ('a \<times> bool \<Rightarrow> 'a MABP) \<Rightarrow> ('a \<times> bool) tstream \<rightarrow> 'a MABP tstream) 
-            BoolPair\<cdot>(tsMed\<cdot>(tsMap invBoolPair\<cdot>(x . ds))\<cdot>bst))"
+            BoolPair\<cdot>(tsMed\<cdot>(tsMap invBoolPair\<cdot>(x . c_ds))\<cdot>bst))"
 
 lemma medsrh_cont [simp]: "cont (medSRH bst)"
   by (simp add: medSRH_def)
@@ -632,7 +616,7 @@ lemma medsrh_contlub: assumes "chain Y"
   apply (rule cont2contlubE)
   by (simp_all add: assms)
 
-lemma to_medsrh: "tsMap BoolPair\<cdot>(tsMed\<cdot>(tsMap invBoolPair\<cdot>(x  .  ds))\<cdot>bst)
+lemma to_medsrh: "tsMap BoolPair\<cdot>(tsMed\<cdot>(tsMap invBoolPair\<cdot>(x  .  c_ds))\<cdot>bst)
                   = ((medSRH :: bool stream \<Rightarrow> 'a MABP TSB \<Rightarrow> 'a MABP tstream) bst) x"
   by (simp add: medSRH_def)
 
@@ -645,40 +629,40 @@ lemma tsmed_input_mono [simp]: "monofun (\<lambda> x. tsMed\<cdot>x\<cdot>bst)"
   using cont2mono tsmed_input_cont by blast
 *)
 
-lemma medsr_tsb_well[simp]: "tsb_well [dr \<mapsto> tsMap BoolPair\<cdot>(tsMed\<cdot>(tsMap invBoolPair\<cdot>(x . ds))\<cdot>bst)]"
+lemma medsr_tsb_well[simp]: "tsb_well [c_dr \<mapsto> tsMap BoolPair\<cdot>(tsMed\<cdot>(tsMap invBoolPair\<cdot>(x . c_ds))\<cdot>bst)]"
   apply (rule tsb_wellI)
   by (simp add: tsmap_tsdom_range)
 
-lemma medsr_tsb_dom: "tsbDom\<cdot>([dr \<mapsto> tsMap BoolPair\<cdot>(tsMed\<cdot>(tsMap invBoolPair\<cdot>(x . ds))\<cdot>bst)]\<Omega>) = {dr}"
+lemma medsr_tsb_dom: "tsbDom\<cdot>([c_dr \<mapsto> tsMap BoolPair\<cdot>(tsMed\<cdot>(tsMap invBoolPair\<cdot>(x . c_ds))\<cdot>bst)]\<Omega>) = {c_dr}"
   by (simp add: tsbdom_rep_eq)
     
   subsubsection \<open>cont\<close>
     
 (* definition tsMedSRTSPF :: "bool stream \<Rightarrow> 'a MABP TSPF" where
-"tsMedSRTSPF bst\<equiv> Abs_CTSPF (\<lambda> x. (tsbDom\<cdot>x = {ds})
-  \<leadsto> [dr \<mapsto> (tsMap:: ('a \<times> bool \<Rightarrow> 'a MABP) \<Rightarrow> ('a \<times> bool) tstream \<rightarrow> 'a MABP tstream) 
-            BoolPair\<cdot>(tsMed\<cdot>(tsMap invBoolPair\<cdot>(x . ds))\<cdot>bst)]\<Omega>)" *)
+"tsMedSRTSPF bst\<equiv> Abs_CTSPF (\<lambda> x. (tsbDom\<cdot>x = {c_ds})
+  \<leadsto> [c_dr \<mapsto> (tsMap:: ('a \<times> bool \<Rightarrow> 'a MABP) \<Rightarrow> ('a \<times> bool) tstream \<rightarrow> 'a MABP tstream) 
+            BoolPair\<cdot>(tsMed\<cdot>(tsMap invBoolPair\<cdot>(x . c_ds))\<cdot>bst)]\<Omega>)" *)
 
 (* this can be shown analogue to before *)
-lemma medsr_cont [simp]: "cont (\<lambda> x::'a MABP TSB. (tsbDom\<cdot>x = {ds})
-  \<leadsto> [dr \<mapsto> (tsMap:: ('a \<times> bool \<Rightarrow> 'a MABP) \<Rightarrow> ('a \<times> bool) tstream \<rightarrow> 'a MABP tstream) 
-            BoolPair\<cdot>(tsMed\<cdot>(tsMap invBoolPair\<cdot>(x . ds))\<cdot>bst)]\<Omega>)"
+lemma medsr_cont [simp]: "cont (\<lambda> x::'a MABP TSB. (tsbDom\<cdot>x = {c_ds})
+  \<leadsto> [c_dr \<mapsto> (tsMap:: ('a \<times> bool \<Rightarrow> 'a MABP) \<Rightarrow> ('a \<times> bool) tstream \<rightarrow> 'a MABP tstream) 
+            BoolPair\<cdot>(tsMed\<cdot>(tsMap invBoolPair\<cdot>(x . c_ds))\<cdot>bst)]\<Omega>)"
   sorry
     
  
   subsubsection \<open>tspf_well\<close>
 
-lemma medsr_tick: assumes "tsbDom\<cdot>b = {ds}" and "(#\<surd>tsb b) = n" and "#bst=\<infinity>"
-  shows "n \<le> (#\<surd>tsb [dr \<mapsto> (tsMap:: ('a \<times> bool \<Rightarrow> 'a MABP) \<Rightarrow> ('a \<times> bool) tstream \<rightarrow> 'a MABP tstream) 
-            BoolPair\<cdot>(tsMed\<cdot>(tsMap invBoolPair\<cdot>(b . ds))\<cdot>bst)]\<Omega>)"
+lemma medsr_tick: assumes "tsbDom\<cdot>b = {c_ds}" and "(#\<surd>tsb b) = n" and "#bst=\<infinity>"
+  shows "n \<le> (#\<surd>tsb [c_dr \<mapsto> (tsMap:: ('a \<times> bool \<Rightarrow> 'a MABP) \<Rightarrow> ('a \<times> bool) tstream \<rightarrow> 'a MABP tstream) 
+            BoolPair\<cdot>(tsMed\<cdot>(tsMap invBoolPair\<cdot>(b . c_ds))\<cdot>bst)]\<Omega>)"
 proof -
-  have "(#\<surd>tsb b) = #\<surd>(b . ds)"
+  have "(#\<surd>tsb b) = #\<surd>(b . c_ds)"
     apply (rule tsbtick_single_ch2)
     by (simp add: assms(1))
-  hence f1: "n = #\<surd>(b . ds)"
+  hence f1: "n = #\<surd>(b . c_ds)"
     using assms(2) by blast
   hence f2: "n \<le> #\<surd>((tsMap:: ('a \<times> bool \<Rightarrow> 'a MABP) \<Rightarrow> ('a \<times> bool) tstream \<rightarrow> 'a MABP tstream) 
-            BoolPair\<cdot>(tsMed\<cdot>(tsMap invBoolPair\<cdot>(b . ds))\<cdot>bst))"
+            BoolPair\<cdot>(tsMed\<cdot>(tsMap invBoolPair\<cdot>(b . c_ds))\<cdot>bst))"
     by (simp add: assms(3))
   show ?thesis
     apply (rule tsbtick_geI)
@@ -688,9 +672,9 @@ qed
     
   (* a medium is a tspf if the oracle bool stream bst is infinitly long*)
 lemma medsr_well [simp]: assumes "#bst=\<infinity>"
-  shows "tspf_well (\<Lambda> x.(tsbDom\<cdot>x = {ds})
-  \<leadsto> [dr \<mapsto> (tsMap:: ('a \<times> bool \<Rightarrow> 'a MABP) \<Rightarrow> ('a \<times> bool) tstream \<rightarrow> 'a MABP tstream) 
-            BoolPair\<cdot>(tsMed\<cdot>(tsMap invBoolPair\<cdot>(x . ds))\<cdot>bst)]\<Omega>)"
+  shows "tspf_well (\<Lambda> x.(tsbDom\<cdot>x = {c_ds})
+  \<leadsto> [c_dr \<mapsto> (tsMap:: ('a \<times> bool \<Rightarrow> 'a MABP) \<Rightarrow> ('a \<times> bool) tstream \<rightarrow> 'a MABP tstream) 
+            BoolPair\<cdot>(tsMed\<cdot>(tsMap invBoolPair\<cdot>(x . c_ds))\<cdot>bst)]\<Omega>)"
   apply (rule tspf_wellI)
     apply (simp_all add: domIff2 medsr_tsb_dom)
     apply (subst tsbtick_single_ch1, simp)
@@ -700,14 +684,14 @@ lemma medsr_revsubst: "Abs_CTSPF (medSR_TSPFAbb bst) = (medSR_TSPF bst)"
   by (simp add: medSR_TSPF_def)
     
 lemma medsr_tspfdom: assumes "#bst =\<infinity>"
-  shows "tspfDom\<cdot>(medSR_TSPF bst) = {ds}"
+  shows "tspfDom\<cdot>(medSR_TSPF bst) = {c_ds}"
     apply (simp add: medSR_TSPF_def)
     apply (simp add: tspf_dom_insert assms)
     apply (simp add: domIff2)
     by (meson tsbleast_tsdom someI)
    
 lemma medsr_tspfran: assumes "#bst =\<infinity>"
-  shows "tspfRan\<cdot>(medSR_TSPF bst) = {dr}"   
+  shows "tspfRan\<cdot>(medSR_TSPF bst) = {c_dr}"   
     apply (simp add: medSR_TSPF_def)
     apply (simp add: tspfran_least medsr_tspfdom assms)
     apply (simp add: medsr_revsubst medsr_tspfdom assms)
@@ -716,9 +700,9 @@ lemma medsr_tspfran: assumes "#bst =\<infinity>"
   (* now special lemmata for TSPS instantiation *)
 
 lemma medsr_well2 [simp]: assumes "#({True} \<ominus> bst) = \<infinity>"
-  shows "tspf_well (\<Lambda> x.(tsbDom\<cdot>x = {ds})
-  \<leadsto> [dr \<mapsto> (tsMap:: ('a \<times> bool \<Rightarrow> 'a MABP) \<Rightarrow> ('a \<times> bool) tstream \<rightarrow> 'a MABP tstream) 
-            BoolPair\<cdot>(tsMed\<cdot>(tsMap invBoolPair\<cdot>(x . ds))\<cdot>bst)]\<Omega>)"
+  shows "tspf_well (\<Lambda> x.(tsbDom\<cdot>x = {c_ds})
+  \<leadsto> [c_dr \<mapsto> (tsMap:: ('a \<times> bool \<Rightarrow> 'a MABP) \<Rightarrow> ('a \<times> bool) tstream \<rightarrow> 'a MABP tstream) 
+            BoolPair\<cdot>(tsMed\<cdot>(tsMap invBoolPair\<cdot>(x . c_ds))\<cdot>bst)]\<Omega>)"
 proof -
    have "#bst = \<infinity>"
      by (simp add: med_ora_length assms(1))
@@ -728,7 +712,7 @@ qed
   
 
 lemma medsr_tspfdom2: assumes "#({True} \<ominus> bst) = \<infinity>"
-  shows "tspfDom\<cdot>(medSR_TSPF bst) = {ds}"
+  shows "tspfDom\<cdot>(medSR_TSPF bst) = {c_ds}"
 proof -
   have "#bst = \<infinity>"
     by (simp add: med_ora_length assms(1))
@@ -737,7 +721,7 @@ proof -
 qed
   
 lemma medsr_tspfran2: assumes "#({True} \<ominus> bst) = \<infinity>"
-  shows "tspfRan\<cdot>(medSR_TSPF bst) = {dr}"
+  shows "tspfRan\<cdot>(medSR_TSPF bst) = {c_dr}"
 proof -
   have "#bst = \<infinity>"
     by (simp add: med_ora_length assms(1))
@@ -746,18 +730,18 @@ proof -
 qed
 
   (* necessary for TSPS instantiation *)
-lemma medsr_tsps_dom1 [simp]: "f = medSR_TSPF ora \<and> #({True} \<ominus> ora) = \<infinity> \<Longrightarrow> tspfDom\<cdot>f = {ds}"
+lemma medsr_tsps_dom1 [simp]: "f = medSR_TSPF ora \<and> #({True} \<ominus> ora) = \<infinity> \<Longrightarrow> tspfDom\<cdot>f = {c_ds}"
   by (simp add: medsr_tspfdom2)
 
 lemma medsr_tsps_dom2 [simp]: "\<exists>ora::bool stream. f = medSR_TSPF ora \<and> #({True} \<ominus> ora) = \<infinity> 
-                               \<Longrightarrow> tspfDom\<cdot>f = {ds}"
+                               \<Longrightarrow> tspfDom\<cdot>f = {c_ds}"
   using medsr_tsps_dom1  by auto
  
-lemma medsr_tsps_ran1 [simp]: "f = medSR_TSPF ora \<and> #({True} \<ominus> ora) = \<infinity> \<Longrightarrow> tspfRan\<cdot>f = {dr}"
+lemma medsr_tsps_ran1 [simp]: "f = medSR_TSPF ora \<and> #({True} \<ominus> ora) = \<infinity> \<Longrightarrow> tspfRan\<cdot>f = {c_dr}"
   by (simp add: medsr_tspfran2)
 
 lemma medsr_tsps_ran2 [simp]: "\<exists>ora::bool stream. f = medSR_TSPF ora \<and> #({True} \<ominus> ora) = \<infinity> 
-                               \<Longrightarrow> tspfRan\<cdot>f = {dr}"
+                               \<Longrightarrow> tspfRan\<cdot>f = {c_dr}"
   using medsr_tsps_ran1 by auto
       
 (* ----------------------------------------------------------------------- *)
@@ -797,8 +781,8 @@ section \<open>More Lemmas\<close>
   
   (* Final lemma for general composition operator*)
 lemma abp_gencomp_final: assumes "f \<in> Rep_TSPS gencompABP"
-                            and "tsbDom\<cdot>tb = {abpIn}"
-  shows "tsAbs\<cdot>((f \<rightleftharpoons> tb) . abpOut) = tsAbs\<cdot>(tb . abpIn)"
+                            and "tsbDom\<cdot>tb = {c_abpIn}"
+  shows "tsAbs\<cdot>((f \<rightleftharpoons> tb) . c_abpOut) = tsAbs\<cdot>(tb . c_abpIn)"
   oops                          
       
 end
